chore: update stage0

stage0/stdlib/Init/Data/List/BasicAux.c
@@ -1,6 +1,6 @@
 // Lean compiler output
 // Module: Init.Data.List.BasicAux
-// Imports: Init.Data.List.Basic Init.Util
+// Imports: Init.Data.Nat.Linear Init.Data.List.Basic Init.Util
 #include <lean/lean.h>
 #if defined(__clang__)
 #pragma clang diagnostic ignored "-Wunused-parameter"
@@ -111,7 +111,7 @@ _start:
 lean_object* x_1; lean_object* x_2; lean_object* x_3; lean_object* x_4; lean_object* x_5; lean_object* x_6; 
 x_1 = l_List_get_x21___rarg___closed__1;
 x_2 = l_List_get_x21___rarg___closed__2;
-x_3 = lean_unsigned_to_nat(19u);
+x_3 = lean_unsigned_to_nat(20u);
 x_4 = lean_unsigned_to_nat(18u);
 x_5 = l_List_get_x21___rarg___closed__3;
 x_6 = l___private_Init_Util_0__mkPanicMessageWithDecl(x_1, x_2, x_3, x_4, x_5);
@@ -289,7 +289,7 @@ _start:
 lean_object* x_1; lean_object* x_2; lean_object* x_3; lean_object* x_4; lean_object* x_5; lean_object* x_6; 
 x_1 = l_List_get_x21___rarg___closed__1;
 x_2 = l_List_head_x21___rarg___closed__1;
-x_3 = lean_unsigned_to_nat(30u);
+x_3 = lean_unsigned_to_nat(31u);
 x_4 = lean_unsigned_to_nat(12u);
 x_5 = l_List_head_x21___rarg___closed__2;
 x_6 = l___private_Init_Util_0__mkPanicMessageWithDecl(x_1, x_2, x_3, x_4, x_5);
@@ -462,7 +462,7 @@ _start:
 lean_object* x_1; lean_object* x_2; lean_object* x_3; lean_object* x_4; lean_object* x_5; lean_object* x_6; 
 x_1 = l_List_get_x21___rarg___closed__1;
 x_2 = l_List_tail_x21___rarg___closed__1;
-x_3 = lean_unsigned_to_nat(45u);
+x_3 = lean_unsigned_to_nat(46u);
 x_4 = lean_unsigned_to_nat(13u);
 x_5 = l_List_head_x21___rarg___closed__2;
 x_6 = l___private_Init_Util_0__mkPanicMessageWithDecl(x_1, x_2, x_3, x_4, x_5);
@@ -634,7 +634,7 @@ _start:
 lean_object* x_1; lean_object* x_2; lean_object* x_3; lean_object* x_4; lean_object* x_5; lean_object* x_6; 
 x_1 = l_List_get_x21___rarg___closed__1;
 x_2 = l_List_getLast_x21___rarg___closed__1;
-x_3 = lean_unsigned_to_nat(62u);
+x_3 = lean_unsigned_to_nat(63u);
 x_4 = lean_unsigned_to_nat(13u);
 x_5 = l_List_head_x21___rarg___closed__2;
 x_6 = l___private_Init_Util_0__mkPanicMessageWithDecl(x_1, x_2, x_3, x_4, x_5);
@@ -877,6 +877,7 @@ lean_dec(x_2);
 return x_3;
 }
 }
+lean_object* initialize_Init_Data_Nat_Linear(uint8_t builtin, lean_object*);
 lean_object* initialize_Init_Data_List_Basic(uint8_t builtin, lean_object*);
 lean_object* initialize_Init_Util(uint8_t builtin, lean_object*);
 static bool _G_initialized = false;
@@ -884,6 +885,9 @@ LEAN_EXPORT lean_object* initialize_Init_Data_List_BasicAux(uint8_t builtin, lea
 lean_object * res;
 if (_G_initialized) return lean_io_result_mk_ok(lean_box(0));
 _G_initialized = true;
+res = initialize_Init_Data_Nat_Linear(builtin, lean_io_mk_world());
+if (lean_io_result_is_error(res)) return res;
+lean_dec_ref(res);
 res = initialize_Init_Data_List_Basic(builtin, lean_io_mk_world());
 if (lean_io_result_is_error(res)) return res;
 lean_dec_ref(res);
