stage0/stdlib/Init/Data/Nat/Basic.c
@@ -41,15 +41,18 @@ LEAN_EXPORT lean_object* l_Prod_anyI___boxed(lean_object*, lean_object*);
 LEAN_EXPORT lean_object* l_Nat_foldRev___rarg(lean_object*, lean_object*, lean_object*);
 LEAN_EXPORT lean_object* l_Nat_anyAux___boxed(lean_object*, lean_object*, lean_object*);
 LEAN_EXPORT uint8_t l_Nat_all(lean_object*, lean_object*);
+LEAN_EXPORT lean_object* l_Nat_blt___boxed(lean_object*, lean_object*);
 LEAN_EXPORT lean_object* l_Nat_anyAux___at_Prod_allI___spec__1___boxed(lean_object*, lean_object*, lean_object*);
 LEAN_EXPORT lean_object* l_Nat_instTransNatLtInstLTNat;
 LEAN_EXPORT lean_object* l_Nat_fold___rarg(lean_object*, lean_object*, lean_object*);
 LEAN_EXPORT lean_object* l_Prod_allI___boxed(lean_object*, lean_object*);
 LEAN_EXPORT uint8_t l_Prod_allI(lean_object*, lean_object*);
 uint8_t lean_nat_dec_le(lean_object*, lean_object*);
+uint8_t lean_nat_dec_le(lean_object*, lean_object*);
 LEAN_EXPORT lean_object* l_Nat_any___boxed(lean_object*, lean_object*);
 LEAN_EXPORT lean_object* l_Nat_repeat___rarg(lean_object*, lean_object*, lean_object*);
 LEAN_EXPORT uint8_t l_Nat_anyAux___at_Nat_all___spec__1(lean_object*, lean_object*, lean_object*);
+LEAN_EXPORT uint8_t l_Nat_blt(lean_object*, lean_object*);
 LEAN_EXPORT lean_object* l_Nat_foldAux___rarg___boxed(lean_object*, lean_object*, lean_object*, lean_object*);
 LEAN_EXPORT uint8_t l_Nat_anyAux(lean_object*, lean_object*, lean_object*);
 LEAN_EXPORT lean_object* l_Nat_min(lean_object*, lean_object*);
@@ -373,6 +376,28 @@ _start:
 lean_object* x_2; 
 x_2 = lean_alloc_closure((void*)(l_Nat_repeat___rarg), 3, 0);
 return x_2;
+}
+}
+LEAN_EXPORT uint8_t l_Nat_blt(lean_object* x_1, lean_object* x_2) {
+_start:
+{
+lean_object* x_3; lean_object* x_4; uint8_t x_5; 
+x_3 = lean_unsigned_to_nat(1u);
+x_4 = lean_nat_add(x_1, x_3);
+x_5 = lean_nat_dec_le(x_4, x_2);
+lean_dec(x_4);
+return x_5;
+}
+}
+LEAN_EXPORT lean_object* l_Nat_blt___boxed(lean_object* x_1, lean_object* x_2) {
+_start:
+{
+uint8_t x_3; lean_object* x_4; 
+x_3 = l_Nat_blt(x_1, x_2);
+lean_dec(x_2);
+lean_dec(x_1);
+x_4 = lean_box(x_3);
+return x_4;
 }
 }
 static lean_object* _init_l_Nat_instTransNatLtInstLTNat() {
