stage0/stdlib/Init/Notation.c
@@ -89,6 +89,8 @@ static lean_object* l_term___u2218_____closed__5;
 static lean_object* l_prec_x28___x29___closed__5;
 static lean_object* l_Lean_Parser_Tactic_case___closed__6;
 static lean_object* l_term___x5e_x5e_x5e_____closed__3;
+static lean_object* l___aux__Init__Notation______macroRules__boolIfThenElse__1___closed__4;
+LEAN_EXPORT lean_object* l___aux__Init__Notation______macroRules__boolIfThenElse__1(lean_object*, lean_object*, lean_object*);
 LEAN_EXPORT lean_object* l_term___x26_x26_x26__;
 static lean_object* l_termMax__prec___closed__2;
 static lean_object* l_Lean_Parser_Tactic___aux__Init__Notation______macroRules__Lean__Parser__Tactic__tacticInfer__instance__1___closed__2;
@@ -100,6 +102,7 @@ static lean_object* l_term___x2d_____closed__1;
 static lean_object* l_termMax__prec___closed__1;
 static lean_object* l_Lean___aux__Init__Notation______macroRules__Lean__termThis__1___closed__2;
 static lean_object* l_precLead___closed__4;
+static lean_object* l_boolIfThenElse___closed__2;
 LEAN_EXPORT lean_object* l_term_x2d__;
 lean_object* lean_mk_empty_array_with_capacity(lean_object*);
 static lean_object* l_term___u2264_____closed__5;
@@ -114,6 +117,7 @@ static lean_object* l_precMax___closed__3;
 LEAN_EXPORT lean_object* l_Lean_Parser_Tactic_refine_x27;
 static lean_object* l___aux__Init__Notation______macroRules__term___x3c_x24_x3e____1___closed__7;
 static lean_object* l_Lean_Parser_Tactic_first___closed__9;
+static lean_object* l_boolIfThenElse___closed__13;
 lean_object* l_Lean_Syntax_getHeadInfo_x3f(lean_object*);
 static lean_object* l___aux__Init__Notation______macroRules__stx___x2c_x2b__1___closed__2;
 static lean_object* l_stx___x3c_x7c_x3e_____closed__2;
@@ -338,6 +342,7 @@ static lean_object* l_Lean_Parser_Tactic_casesTarget___closed__4;
 static lean_object* l_Lean_Parser_Tactic_tacticHave_____closed__3;
 static lean_object* l___aux__Init__Notation______macroRules__stx___x2b__1___closed__1;
 static lean_object* l_Lean_Parser_Tactic_unfold___closed__4;
+static lean_object* l_boolIfThenElse___closed__6;
 static lean_object* l_Lean_Parser_Tactic_change___closed__1;
 static lean_object* l_Lean_Parser_Tactic_tacticRefine__lift_____closed__5;
 static lean_object* l_Lean_Parser_Tactic_intro___closed__13;
@@ -535,6 +540,7 @@ static lean_object* l_termIfLet___x3a_x3d__Then__Else_____closed__14;
 static lean_object* l_Lean_Parser_Tactic_intros___closed__6;
 static lean_object* l_prec_x28___x29___closed__2;
 static lean_object* l_Lean_Parser_Tactic_first___closed__12;
+static lean_object* l_boolIfThenElse___closed__10;
 LEAN_EXPORT lean_object* l_Lean_Parser_Tactic_contradiction;
 static lean_object* l___aux__Init__Notation______macroRules__term___x2b____1___closed__6;
 static lean_object* l_termDepIfThenElse___closed__37;
@@ -587,6 +593,7 @@ static lean_object* l___aux__Init__Notation______macroRules__term___x2a_x3e____1
 static lean_object* l_Lean_Parser_Tactic_tacticNext_______x3d_x3e_____closed__5;
 LEAN_EXPORT lean_object* l___aux__Init__Notation______macroRules__prio_x28___x29__1(lean_object*, lean_object*, lean_object*);
 static lean_object* l___aux__Init__Notation______macroRules__term___x2f_x5c____1___closed__4;
+static lean_object* l_boolIfThenElse___closed__14;
 LEAN_EXPORT lean_object* l_Lean_Parser_Tactic___aux__Init__Notation______macroRules__Lean__Parser__Tactic__tactic___x3c_x3b_x3e____1(lean_object*, lean_object*, lean_object*);
 static lean_object* l_term___x3c_x7c_____closed__3;
 static lean_object* l_prioDefault___closed__4;
@@ -653,6 +660,7 @@ static lean_object* l_term___x7c_x7c_x7c_____closed__6;
 static lean_object* l_term___x5c_x2f_____closed__5;
 static lean_object* l_term___u2264_____closed__1;
 static lean_object* l___aux__Init__Notation______macroRules__term___x3e_x3e____1___closed__7;
+static lean_object* l_boolIfThenElse___closed__3;
 static lean_object* l_Lean_Parser_Tactic_inductionAlt___closed__10;
 LEAN_EXPORT lean_object* l___aux__Init__Notation______unexpand__LE__le__1___boxed(lean_object*, lean_object*, lean_object*);
 static lean_object* l_Lean_Parser_Tactic_config___closed__7;
@@ -681,6 +689,7 @@ LEAN_EXPORT lean_object* l___aux__Init__Notation______macroRules__term___x3c_x3d
 static lean_object* l_term___u2227_____closed__1;
 static lean_object* l___aux__Init__Notation______macroRules__term___x2f____1___closed__2;
 static lean_object* l___aux__Init__Notation______macroRules__stx___x2a__1___closed__1;
+static lean_object* l_boolIfThenElse___closed__5;
 static lean_object* l_Lean_Parser_Attr_simp___closed__3;
 static lean_object* l_Lean_Parser_Tactic_rename___closed__10;
 static lean_object* l_Lean_Parser_Tactic_locationHyp___closed__3;
@@ -874,6 +883,7 @@ LEAN_EXPORT lean_object* l_Lean_Parser_Tactic___aux__Init__Notation______macroRu
 static lean_object* l_Lean_Parser_Tactic_changeWith___closed__1;
 static lean_object* l___aux__Init__Notation______macroRules__term_x21____1___closed__2;
 static lean_object* l_Lean_Parser_Syntax_addPrio___closed__1;
+static lean_object* l_boolIfThenElse___closed__7;
 static lean_object* l_term___x7c_x7c_x7c_____closed__5;
 static lean_object* l_termIfThenElse___closed__1;
 lean_object* l_Lean_replaceRef(lean_object*, lean_object*);
@@ -1294,6 +1304,7 @@ static lean_object* l_Lean_Parser_Tactic_fail___closed__4;
 static lean_object* l_Lean_Parser_Tactic_subst___closed__5;
 static lean_object* l_Lean_Parser_Tactic_inductionAlt___closed__5;
 LEAN_EXPORT lean_object* l_Lean_Parser_Tactic_subst;
+static lean_object* l___aux__Init__Notation______macroRules__boolIfThenElse__1___closed__5;
 static lean_object* l_termDepIfThenElse___closed__22;
 static lean_object* l_term___u2265_____closed__3;
 static lean_object* l___aux__Init__Notation______macroRules__term___x3c____1___closed__1;
@@ -1364,6 +1375,7 @@ static lean_object* l_Lean_Parser_Tactic___aux__Init__Notation______macroRules__
 static lean_object* l_term___x3c_x2a_x3e_____closed__6;
 static lean_object* l_term_x2d_____closed__3;
 static lean_object* l_precMin___closed__4;
+static lean_object* l___aux__Init__Notation______macroRules__boolIfThenElse__1___closed__3;
 static lean_object* l_Lean_Parser_Tactic_tacticHave_x27_____x3a_x3d_____closed__2;
 static lean_object* l_Lean_Parser_Tactic_tacticLet_x27_____closed__3;
 static lean_object* l_Lean_Parser_Tactic_existsIntro___closed__6;
@@ -1415,6 +1427,7 @@ LEAN_EXPORT lean_object* l_Lean_Parser_Tactic___aux__Init__Notation______macroRu
 static lean_object* l_Lean_Parser_Tactic_tacticNext_______x3d_x3e_____closed__9;
 static lean_object* l_Lean___aux__Init__Notation______macroRules__term_x5b___x5d__1___closed__1;
 static lean_object* l___aux__Init__Notation______macroRules__term___x3c____1___closed__9;
+static lean_object* l_boolIfThenElse___closed__12;
 static lean_object* l_Lean_Parser_Tactic_tacticLet_x27_____closed__6;
 static lean_object* l_Lean_Parser_Tactic_refine___closed__2;
 static lean_object* l___aux__Init__Notation______macroRules__term___x3d_x3d____2___closed__3;
@@ -1638,6 +1651,7 @@ static lean_object* l_Lean_Parser_Tactic_rename___closed__4;
 LEAN_EXPORT lean_object* l_term___x3e_x3e__;
 static lean_object* l_termMax__prec___closed__5;
 static lean_object* l___aux__Init__Notation______macroRules__prioLow__1___closed__1;
+static lean_object* l___aux__Init__Notation______macroRules__boolIfThenElse__1___closed__6;
 static lean_object* l_Lean_Parser_Tactic___aux__Init__Notation______macroRules__Lean__Parser__Tactic__tacticTry____1___closed__2;
 static lean_object* l___aux__Init__Notation______macroRules__term_u2039___u203a__1___closed__3;
 static lean_object* l_term_x5b___x5d___closed__8;
@@ -1694,6 +1708,7 @@ static lean_object* l_Lean_Parser_Tactic_tacticHave_x27_____closed__2;
 static lean_object* l_term___x2b_____closed__5;
 static lean_object* l_Lean_Parser_Tactic_tacticSuffices_____closed__6;
 static lean_object* l_Lean_Parser_Tactic_renameI___closed__3;
+static lean_object* l_boolIfThenElse___closed__11;
 static lean_object* l___aux__Init__Notation______macroRules__term___x3e_x3e_x3e____1___closed__8;
 LEAN_EXPORT lean_object* l___aux__Init__Notation______macroRules__prec_x28___x29__1___boxed(lean_object*, lean_object*, lean_object*);
 static lean_object* l_Lean_Parser_Tactic_induction___closed__14;
@@ -1941,6 +1956,7 @@ static lean_object* l_Lean_Parser_Tactic_simpLemma___closed__5;
 LEAN_EXPORT lean_object* l___aux__Init__Notation______macroRules__stx___x2c_x2b__1(lean_object*, lean_object*, lean_object*);
 static lean_object* l_Lean_Parser_Tactic_simpPost___closed__3;
 static lean_object* l_Lean_Parser_Tactic_intro___closed__3;
+LEAN_EXPORT lean_object* l_boolIfThenElse;
 LEAN_EXPORT lean_object* l___aux__Init__Notation______unexpand__not__1(lean_object*, lean_object*, lean_object*);
 static lean_object* l_Lean_Parser_Tactic_discharger___closed__7;
 static lean_object* l___aux__Init__Notation______macroRules__term___x3c_x2a_x3e____1___closed__1;
@@ -2016,8 +2032,10 @@ static lean_object* l___aux__Init__Notation______macroRules__stx___x3c_x7c_x3e__
 static lean_object* l_termIfLet___x3a_x3d__Then__Else_____closed__1;
 static lean_object* l___aux__Init__Notation______macroRules__term_x21____1___closed__3;
 static lean_object* l_term___x3e_____closed__5;
+static lean_object* l___aux__Init__Notation______macroRules__boolIfThenElse__1___closed__2;
 static lean_object* l_Lean_Parser_Tactic_existsIntro___closed__1;
 LEAN_EXPORT lean_object* l___aux__Init__Notation______unexpand__LE__le__2(lean_object*, lean_object*, lean_object*);
+static lean_object* l_boolIfThenElse___closed__8;
 static lean_object* l___aux__Init__Notation______macroRules__term___x2d____1___closed__6;
 static lean_object* l___aux__Init__Notation______macroRules__term___x26_x26_x26____1___closed__1;
 static lean_object* l_Lean_Parser_Tactic_tacticRefine__lift_____closed__1;
@@ -2035,6 +2053,7 @@ static lean_object* l_Lean_Parser_Tactic_tacticRefine__lift_____closed__2;
 static lean_object* l_Lean_Parser_Tactic_tacticHave_____x3a_x3d_____closed__7;
 static lean_object* l_prio_x28___x29___closed__1;
 static lean_object* l___aux__Init__Notation______macroRules__term___x3c_x3d____2___closed__2;
+static lean_object* l_boolIfThenElse___closed__4;
 LEAN_EXPORT lean_object* l___aux__Init__Notation______macroRules__term___x3d_x3d____2(lean_object*, lean_object*, lean_object*);
 LEAN_EXPORT lean_object* l_Lean_Parser_Tactic_tacticSuffices__;
 static lean_object* l___aux__Init__Notation______macroRules__term___x3c_x2a_x3e____1___closed__8;
@@ -2058,6 +2077,7 @@ static lean_object* l_Lean_Parser_Tactic_constructor___closed__1;
 static lean_object* l_Lean_Parser_Tactic_tacticHave_x27_____closed__1;
 static lean_object* l_Lean_Parser_Tactic_tacticHave_x27_____x3a_x3d_____closed__4;
 LEAN_EXPORT lean_object* l_Lean_Parser_Tactic_locationHyp;
+static lean_object* l_boolIfThenElse___closed__9;
 static lean_object* l___aux__Init__Notation______macroRules__termWithout__expected__type____1___closed__5;
 static lean_object* l___aux__Init__Notation______macroRules__term_x21____1___closed__5;
 static lean_object* l___aux__Init__Notation______macroRules__term___x7c_x7c_x7c____1___closed__6;
@@ -2066,6 +2086,7 @@ LEAN_EXPORT lean_object* l_Lean_Parser_Tactic_refine;
 static lean_object* l_Lean_Parser_Tactic_rwSeq___closed__6;
 static lean_object* l_term___x3c_x3c_x3c_____closed__4;
 static lean_object* l_Lean_Parser_Tactic_tacticSuffices_____closed__2;
+static lean_object* l_boolIfThenElse___closed__1;
 static lean_object* l_Lean_Parser_Tactic_config___closed__1;
 static lean_object* l___aux__Init__Notation______macroRules__term___x2b____1___closed__1;
 static lean_object* l_term_x7e_x7e_x7e_____closed__4;
@@ -2129,6 +2150,7 @@ static lean_object* l_termIfLet___x3a_x3d__Then__Else_____closed__9;
 static lean_object* l_term___x25_____closed__6;
 LEAN_EXPORT lean_object* l_term___x25__;
 static lean_object* l_stx___x2b___closed__5;
+static lean_object* l___aux__Init__Notation______macroRules__boolIfThenElse__1___closed__1;
 static lean_object* l_Lean_Parser_Tactic_simpPost___closed__1;
 static lean_object* l_Lean_Parser_Tactic___aux__Init__Notation______macroRules__Lean__Parser__Tactic__tacticUnhygienic____1___closed__8;
 static lean_object* l_Lean_Parser_Tactic___aux__Init__Notation______macroRules__Lean__Parser__Tactic__tacticTrivial__5___closed__1;
@@ -26854,6 +26876,367 @@ return x_129;
 }
 }
 }
+static lean_object* _init_l_boolIfThenElse___closed__1() {
+_start:
+{
+lean_object* x_1; 
+x_1 = lean_mk_string("boolIfThenElse");
+return x_1;
+}
+}
+static lean_object* _init_l_boolIfThenElse___closed__2() {
+_start:
+{
+lean_object* x_1; lean_object* x_2; lean_object* x_3; 
+x_1 = lean_box(0);
+x_2 = l_boolIfThenElse___closed__1;
+x_3 = lean_name_mk_string(x_1, x_2);
+return x_3;
+}
+}
+static lean_object* _init_l_boolIfThenElse___closed__3() {
+_start:
+{
+lean_object* x_1; 
+x_1 = lean_mk_string("bif ");
+return x_1;
+}
+}
+static lean_object* _init_l_boolIfThenElse___closed__4() {
+_start:
+{
+lean_object* x_1; lean_object* x_2; 
+x_1 = l_boolIfThenElse___closed__3;
+x_2 = lean_alloc_ctor(5, 1, 0);
+lean_ctor_set(x_2, 0, x_1);
+return x_2;
+}
+}
+static lean_object* _init_l_boolIfThenElse___closed__5() {
+_start:
+{
+lean_object* x_1; lean_object* x_2; lean_object* x_3; lean_object* x_4; 
+x_1 = l_Lean_Parser_Syntax_addPrec___closed__10;
+x_2 = l_boolIfThenElse___closed__4;
+x_3 = l_termDepIfThenElse___closed__16;
+x_4 = lean_alloc_ctor(2, 3, 0);
+lean_ctor_set(x_4, 0, x_1);
+lean_ctor_set(x_4, 1, x_2);
+lean_ctor_set(x_4, 2, x_3);
+return x_4;
+}
+}
+static lean_object* _init_l_boolIfThenElse___closed__6() {
+_start:
+{
+lean_object* x_1; lean_object* x_2; lean_object* x_3; lean_object* x_4; 
+x_1 = l_Lean_Parser_Syntax_addPrec___closed__10;
+x_2 = l_boolIfThenElse___closed__5;
+x_3 = l_termDepIfThenElse___closed__19;
+x_4 = lean_alloc_ctor(2, 3, 0);
+lean_ctor_set(x_4, 0, x_1);
+lean_ctor_set(x_4, 1, x_2);
+lean_ctor_set(x_4, 2, x_3);
+return x_4;
+}
+}
+static lean_object* _init_l_boolIfThenElse___closed__7() {
+_start:
+{
+lean_object* x_1; lean_object* x_2; lean_object* x_3; 
+x_1 = l_termDepIfThenElse___closed__8;
+x_2 = l_boolIfThenElse___closed__6;
+x_3 = lean_alloc_ctor(1, 2, 0);
+lean_ctor_set(x_3, 0, x_1);
+lean_ctor_set(x_3, 1, x_2);
+return x_3;
+}
+}
+static lean_object* _init_l_boolIfThenElse___closed__8() {
+_start:
+{
+lean_object* x_1; lean_object* x_2; lean_object* x_3; lean_object* x_4; 
+x_1 = l_Lean_Parser_Syntax_addPrec___closed__10;
+x_2 = l_boolIfThenElse___closed__7;
+x_3 = l_termDepIfThenElse___closed__24;
+x_4 = lean_alloc_ctor(2, 3, 0);
+lean_ctor_set(x_4, 0, x_1);
+lean_ctor_set(x_4, 1, x_2);
+lean_ctor_set(x_4, 2, x_3);
+return x_4;
+}
+}
+static lean_object* _init_l_boolIfThenElse___closed__9() {
+_start:
+{
+lean_object* x_1; lean_object* x_2; lean_object* x_3; lean_object* x_4; 
+x_1 = l_Lean_Parser_Syntax_addPrec___closed__10;
+x_2 = l_boolIfThenElse___closed__8;
+x_3 = l_termDepIfThenElse___closed__16;
+x_4 = lean_alloc_ctor(2, 3, 0);
+lean_ctor_set(x_4, 0, x_1);
+lean_ctor_set(x_4, 1, x_2);
+lean_ctor_set(x_4, 2, x_3);
+return x_4;
+}
+}
+static lean_object* _init_l_boolIfThenElse___closed__10() {
+_start:
+{
+lean_object* x_1; lean_object* x_2; lean_object* x_3; 
+x_1 = l_termDepIfThenElse___closed__6;
+x_2 = l_boolIfThenElse___closed__9;
+x_3 = lean_alloc_ctor(1, 2, 0);
+lean_ctor_set(x_3, 0, x_1);
+lean_ctor_set(x_3, 1, x_2);
+return x_3;
+}
+}
+static lean_object* _init_l_boolIfThenElse___closed__11() {
+_start:
+{
+lean_object* x_1; lean_object* x_2; lean_object* x_3; lean_object* x_4; 
+x_1 = l_Lean_Parser_Syntax_addPrec___closed__10;
+x_2 = l_boolIfThenElse___closed__10;
+x_3 = l_termDepIfThenElse___closed__30;
+x_4 = lean_alloc_ctor(2, 3, 0);
+lean_ctor_set(x_4, 0, x_1);
+lean_ctor_set(x_4, 1, x_2);
+lean_ctor_set(x_4, 2, x_3);
+return x_4;
+}
+}
+static lean_object* _init_l_boolIfThenElse___closed__12() {
+_start:
+{
+lean_object* x_1; lean_object* x_2; lean_object* x_3; lean_object* x_4; 
+x_1 = l_Lean_Parser_Syntax_addPrec___closed__10;
+x_2 = l_boolIfThenElse___closed__11;
+x_3 = l_termDepIfThenElse___closed__35;
+x_4 = lean_alloc_ctor(2, 3, 0);
+lean_ctor_set(x_4, 0, x_1);
+lean_ctor_set(x_4, 1, x_2);
+lean_ctor_set(x_4, 2, x_3);
+return x_4;
+}
+}
+static lean_object* _init_l_boolIfThenElse___closed__13() {
+_start:
+{
+lean_object* x_1; lean_object* x_2; lean_object* x_3; 
+x_1 = l_termDepIfThenElse___closed__4;
+x_2 = l_boolIfThenElse___closed__12;
+x_3 = lean_alloc_ctor(1, 2, 0);
+lean_ctor_set(x_3, 0, x_1);
+lean_ctor_set(x_3, 1, x_2);
+return x_3;
+}
+}
+static lean_object* _init_l_boolIfThenElse___closed__14() {
+_start:
+{
+lean_object* x_1; lean_object* x_2; lean_object* x_3; lean_object* x_4; 
+x_1 = l_boolIfThenElse___closed__2;
+x_2 = lean_unsigned_to_nat(1022u);
+x_3 = l_boolIfThenElse___closed__13;
+x_4 = lean_alloc_ctor(3, 3, 0);
+lean_ctor_set(x_4, 0, x_1);
+lean_ctor_set(x_4, 1, x_2);
+lean_ctor_set(x_4, 2, x_3);
+return x_4;
+}
+}
+static lean_object* _init_l_boolIfThenElse() {
+_start:
+{
+lean_object* x_1; 
+x_1 = l_boolIfThenElse___closed__14;
+return x_1;
+}
+}
+static lean_object* _init_l___aux__Init__Notation______macroRules__boolIfThenElse__1___closed__1() {
+_start:
+{
+lean_object* x_1; 
+x_1 = lean_mk_string("cond");
+return x_1;
+}
+}
+static lean_object* _init_l___aux__Init__Notation______macroRules__boolIfThenElse__1___closed__2() {
+_start:
+{
+lean_object* x_1; lean_object* x_2; 
+x_1 = l___aux__Init__Notation______macroRules__boolIfThenElse__1___closed__1;
+x_2 = lean_string_utf8_byte_size(x_1);
+return x_2;
+}
+}
+static lean_object* _init_l___aux__Init__Notation______macroRules__boolIfThenElse__1___closed__3() {
+_start:
+{
+lean_object* x_1; lean_object* x_2; lean_object* x_3; lean_object* x_4; 
+x_1 = l___aux__Init__Notation______macroRules__boolIfThenElse__1___closed__1;
+x_2 = lean_unsigned_to_nat(0u);
+x_3 = l___aux__Init__Notation______macroRules__boolIfThenElse__1___closed__2;
+x_4 = lean_alloc_ctor(0, 3, 0);
+lean_ctor_set(x_4, 0, x_1);
+lean_ctor_set(x_4, 1, x_2);
+lean_ctor_set(x_4, 2, x_3);
+return x_4;
+}
+}
+static lean_object* _init_l___aux__Init__Notation______macroRules__boolIfThenElse__1___closed__4() {
+_start:
+{
+lean_object* x_1; lean_object* x_2; lean_object* x_3; 
+x_1 = lean_box(0);
+x_2 = l___aux__Init__Notation______macroRules__boolIfThenElse__1___closed__1;
+x_3 = lean_name_mk_string(x_1, x_2);
+return x_3;
+}
+}
+static lean_object* _init_l___aux__Init__Notation______macroRules__boolIfThenElse__1___closed__5() {
+_start:
+{
+lean_object* x_1; lean_object* x_2; lean_object* x_3; 
+x_1 = lean_box(0);
+x_2 = l___aux__Init__Notation______macroRules__boolIfThenElse__1___closed__4;
+x_3 = lean_alloc_ctor(0, 2, 0);
+lean_ctor_set(x_3, 0, x_2);
+lean_ctor_set(x_3, 1, x_1);
+return x_3;
+}
+}
+static lean_object* _init_l___aux__Init__Notation______macroRules__boolIfThenElse__1___closed__6() {
+_start:
+{
+lean_object* x_1; lean_object* x_2; lean_object* x_3; 
+x_1 = lean_box(0);
+x_2 = l___aux__Init__Notation______macroRules__boolIfThenElse__1___closed__5;
+x_3 = lean_alloc_ctor(1, 2, 0);
+lean_ctor_set(x_3, 0, x_2);
+lean_ctor_set(x_3, 1, x_1);
+return x_3;
+}
+}
+LEAN_EXPORT lean_object* l___aux__Init__Notation______macroRules__boolIfThenElse__1(lean_object* x_1, lean_object* x_2, lean_object* x_3) {
+_start:
+{
+lean_object* x_4; uint8_t x_5; 
+x_4 = l_boolIfThenElse___closed__2;
+lean_inc(x_1);
+x_5 = l_Lean_Syntax_isOfKind(x_1, x_4);
+if (x_5 == 0)
+{
+lean_object* x_6; lean_object* x_7; 
+lean_dec(x_2);
+lean_dec(x_1);
+x_6 = lean_box(1);
+x_7 = lean_alloc_ctor(1, 2, 0);
+lean_ctor_set(x_7, 0, x_6);
+lean_ctor_set(x_7, 1, x_3);
+return x_7;
+}
+else
+{
+lean_object* x_8; lean_object* x_9; lean_object* x_10; lean_object* x_11; lean_object* x_12; lean_object* x_13; lean_object* x_14; uint8_t x_15; 
+x_8 = lean_unsigned_to_nat(1u);
+x_9 = l_Lean_Syntax_getArg(x_1, x_8);
+x_10 = lean_unsigned_to_nat(3u);
+x_11 = l_Lean_Syntax_getArg(x_1, x_10);
+x_12 = lean_unsigned_to_nat(5u);
+x_13 = l_Lean_Syntax_getArg(x_1, x_12);
+lean_dec(x_1);
+lean_inc(x_2);
+x_14 = l_Lean_MonadRef_mkInfoFromRefPos___at___aux__Init__Notation______macroRules__precMax__1___spec__1(x_2, x_3);
+x_15 = !lean_is_exclusive(x_14);
+if (x_15 == 0)
+{
+lean_object* x_16; lean_object* x_17; lean_object* x_18; lean_object* x_19; lean_object* x_20; lean_object* x_21; lean_object* x_22; lean_object* x_23; lean_object* x_24; lean_object* x_25; lean_object* x_26; lean_object* x_27; lean_object* x_28; lean_object* x_29; lean_object* x_30; lean_object* x_31; lean_object* x_32; lean_object* x_33; lean_object* x_34; lean_object* x_35; 
+x_16 = lean_ctor_get(x_14, 0);
+x_17 = lean_ctor_get(x_2, 2);
+lean_inc(x_17);
+x_18 = lean_ctor_get(x_2, 1);
+lean_inc(x_18);
+lean_dec(x_2);
+x_19 = l___aux__Init__Notation______macroRules__boolIfThenElse__1___closed__4;
+x_20 = l_Lean_addMacroScope(x_18, x_19, x_17);
+x_21 = l___aux__Init__Notation______macroRules__boolIfThenElse__1___closed__3;
+x_22 = l___aux__Init__Notation______macroRules__boolIfThenElse__1___closed__6;
+x_23 = lean_alloc_ctor(3, 4, 0);
+lean_ctor_set(x_23, 0, x_16);
+lean_ctor_set(x_23, 1, x_21);
+lean_ctor_set(x_23, 2, x_20);
+lean_ctor_set(x_23, 3, x_22);
+x_24 = l___aux__Init__Notation______unexpand__Function__comp__1___closed__3;
+x_25 = lean_array_push(x_24, x_9);
+x_26 = lean_array_push(x_25, x_11);
+x_27 = lean_array_push(x_26, x_13);
+x_28 = lean_box(2);
+x_29 = l___aux__Init__Notation______macroRules__stx___x2b__1___closed__8;
+x_30 = lean_alloc_ctor(1, 3, 0);
+lean_ctor_set(x_30, 0, x_28);
+lean_ctor_set(x_30, 1, x_29);
+lean_ctor_set(x_30, 2, x_27);
+x_31 = l___aux__Init__Notation______macroRules__stx___x2c_x2a__1___closed__10;
+x_32 = lean_array_push(x_31, x_23);
+x_33 = lean_array_push(x_32, x_30);
+x_34 = l___aux__Init__Notation______macroRules__term___u2218____1___closed__4;
+x_35 = lean_alloc_ctor(1, 3, 0);
+lean_ctor_set(x_35, 0, x_28);
+lean_ctor_set(x_35, 1, x_34);
+lean_ctor_set(x_35, 2, x_33);
+lean_ctor_set(x_14, 0, x_35);
+return x_14;
+}
+else
+{
+lean_object* x_36; lean_object* x_37; lean_object* x_38; lean_object* x_39; lean_object* x_40; lean_object* x_41; lean_object* x_42; lean_object* x_43; lean_object* x_44; lean_object* x_45; lean_object* x_46; lean_object* x_47; lean_object* x_48; lean_object* x_49; lean_object* x_50; lean_object* x_51; lean_object* x_52; lean_object* x_53; lean_object* x_54; lean_object* x_55; lean_object* x_56; lean_object* x_57; 
+x_36 = lean_ctor_get(x_14, 0);
+x_37 = lean_ctor_get(x_14, 1);
+lean_inc(x_37);
+lean_inc(x_36);
+lean_dec(x_14);
+x_38 = lean_ctor_get(x_2, 2);
+lean_inc(x_38);
+x_39 = lean_ctor_get(x_2, 1);
+lean_inc(x_39);
+lean_dec(x_2);
+x_40 = l___aux__Init__Notation______macroRules__boolIfThenElse__1___closed__4;
+x_41 = l_Lean_addMacroScope(x_39, x_40, x_38);
+x_42 = l___aux__Init__Notation______macroRules__boolIfThenElse__1___closed__3;
+x_43 = l___aux__Init__Notation______macroRules__boolIfThenElse__1___closed__6;
+x_44 = lean_alloc_ctor(3, 4, 0);
+lean_ctor_set(x_44, 0, x_36);
+lean_ctor_set(x_44, 1, x_42);
+lean_ctor_set(x_44, 2, x_41);
+lean_ctor_set(x_44, 3, x_43);
+x_45 = l___aux__Init__Notation______unexpand__Function__comp__1___closed__3;
+x_46 = lean_array_push(x_45, x_9);
+x_47 = lean_array_push(x_46, x_11);
+x_48 = lean_array_push(x_47, x_13);
+x_49 = lean_box(2);
+x_50 = l___aux__Init__Notation______macroRules__stx___x2b__1___closed__8;
+x_51 = lean_alloc_ctor(1, 3, 0);
+lean_ctor_set(x_51, 0, x_49);
+lean_ctor_set(x_51, 1, x_50);
+lean_ctor_set(x_51, 2, x_48);
+x_52 = l___aux__Init__Notation______macroRules__stx___x2c_x2a__1___closed__10;
+x_53 = lean_array_push(x_52, x_44);
+x_54 = lean_array_push(x_53, x_51);
+x_55 = l___aux__Init__Notation______macroRules__term___u2218____1___closed__4;
+x_56 = lean_alloc_ctor(1, 3, 0);
+lean_ctor_set(x_56, 0, x_49);
+lean_ctor_set(x_56, 1, x_55);
+lean_ctor_set(x_56, 2, x_54);
+x_57 = lean_alloc_ctor(0, 2, 0);
+lean_ctor_set(x_57, 0, x_56);
+lean_ctor_set(x_57, 1, x_37);
+return x_57;
+}
+}
+}
+}
 static lean_object* _init_l_term___x3c_x7c_____closed__1() {
 _start:
 {
@@ -46173,6 +46556,48 @@ l___aux__Init__Notation______macroRules__termIfLet___x3a_x3d__Then__Else____1___
 lean_mark_persistent(l___aux__Init__Notation______macroRules__termIfLet___x3a_x3d__Then__Else____1___closed__10);
 l___aux__Init__Notation______macroRules__termIfLet___x3a_x3d__Then__Else____1___closed__11 = _init_l___aux__Init__Notation______macroRules__termIfLet___x3a_x3d__Then__Else____1___closed__11();
 lean_mark_persistent(l___aux__Init__Notation______macroRules__termIfLet___x3a_x3d__Then__Else____1___closed__11);
+l_boolIfThenElse___closed__1 = _init_l_boolIfThenElse___closed__1();
+lean_mark_persistent(l_boolIfThenElse___closed__1);
+l_boolIfThenElse___closed__2 = _init_l_boolIfThenElse___closed__2();
+lean_mark_persistent(l_boolIfThenElse___closed__2);
+l_boolIfThenElse___closed__3 = _init_l_boolIfThenElse___closed__3();
+lean_mark_persistent(l_boolIfThenElse___closed__3);
+l_boolIfThenElse___closed__4 = _init_l_boolIfThenElse___closed__4();
+lean_mark_persistent(l_boolIfThenElse___closed__4);
+l_boolIfThenElse___closed__5 = _init_l_boolIfThenElse___closed__5();
+lean_mark_persistent(l_boolIfThenElse___closed__5);
+l_boolIfThenElse___closed__6 = _init_l_boolIfThenElse___closed__6();
+lean_mark_persistent(l_boolIfThenElse___closed__6);
+l_boolIfThenElse___closed__7 = _init_l_boolIfThenElse___closed__7();
+lean_mark_persistent(l_boolIfThenElse___closed__7);
+l_boolIfThenElse___closed__8 = _init_l_boolIfThenElse___closed__8();
+lean_mark_persistent(l_boolIfThenElse___closed__8);
+l_boolIfThenElse___closed__9 = _init_l_boolIfThenElse___closed__9();
+lean_mark_persistent(l_boolIfThenElse___closed__9);
+l_boolIfThenElse___closed__10 = _init_l_boolIfThenElse___closed__10();
+lean_mark_persistent(l_boolIfThenElse___closed__10);
+l_boolIfThenElse___closed__11 = _init_l_boolIfThenElse___closed__11();
+lean_mark_persistent(l_boolIfThenElse___closed__11);
+l_boolIfThenElse___closed__12 = _init_l_boolIfThenElse___closed__12();
+lean_mark_persistent(l_boolIfThenElse___closed__12);
+l_boolIfThenElse___closed__13 = _init_l_boolIfThenElse___closed__13();
+lean_mark_persistent(l_boolIfThenElse___closed__13);
+l_boolIfThenElse___closed__14 = _init_l_boolIfThenElse___closed__14();
+lean_mark_persistent(l_boolIfThenElse___closed__14);
+l_boolIfThenElse = _init_l_boolIfThenElse();
+lean_mark_persistent(l_boolIfThenElse);
+l___aux__Init__Notation______macroRules__boolIfThenElse__1___closed__1 = _init_l___aux__Init__Notation______macroRules__boolIfThenElse__1___closed__1();
+lean_mark_persistent(l___aux__Init__Notation______macroRules__boolIfThenElse__1___closed__1);
+l___aux__Init__Notation______macroRules__boolIfThenElse__1___closed__2 = _init_l___aux__Init__Notation______macroRules__boolIfThenElse__1___closed__2();
+lean_mark_persistent(l___aux__Init__Notation______macroRules__boolIfThenElse__1___closed__2);
+l___aux__Init__Notation______macroRules__boolIfThenElse__1___closed__3 = _init_l___aux__Init__Notation______macroRules__boolIfThenElse__1___closed__3();
+lean_mark_persistent(l___aux__Init__Notation______macroRules__boolIfThenElse__1___closed__3);
+l___aux__Init__Notation______macroRules__boolIfThenElse__1___closed__4 = _init_l___aux__Init__Notation______macroRules__boolIfThenElse__1___closed__4();
+lean_mark_persistent(l___aux__Init__Notation______macroRules__boolIfThenElse__1___closed__4);
+l___aux__Init__Notation______macroRules__boolIfThenElse__1___closed__5 = _init_l___aux__Init__Notation______macroRules__boolIfThenElse__1___closed__5();
+lean_mark_persistent(l___aux__Init__Notation______macroRules__boolIfThenElse__1___closed__5);
+l___aux__Init__Notation______macroRules__boolIfThenElse__1___closed__6 = _init_l___aux__Init__Notation______macroRules__boolIfThenElse__1___closed__6();
+lean_mark_persistent(l___aux__Init__Notation______macroRules__boolIfThenElse__1___closed__6);
 l_term___x3c_x7c_____closed__1 = _init_l_term___x3c_x7c_____closed__1();
 lean_mark_persistent(l_term___x3c_x7c_____closed__1);
 l_term___x3c_x7c_____closed__2 = _init_l_term___x3c_x7c_____closed__2();
