stage0/stdlib/Lean/Meta/SynthInstance.c
@@ -626,7 +626,7 @@ static lean_object* _init_l_Lean_Meta_initFn____x40_Lean_Meta_SynthInstance___hy
 _start:
 {
 lean_object* x_1; lean_object* x_2; lean_object* x_3; lean_object* x_4; 
-x_1 = lean_unsigned_to_nat(500u);
+x_1 = lean_unsigned_to_nat(20000u);
 x_2 = l_Lean_Meta_initFn____x40_Lean_Meta_SynthInstance___hyg_6____closed__5;
 x_3 = l_Lean_Meta_initFn____x40_Lean_Meta_SynthInstance___hyg_6____closed__6;
 x_4 = lean_alloc_ctor(0, 3, 0);
