stage0/stdlib/Lean/Meta/Tactic/LinearArith/Nat.c
@@ -150,7 +150,7 @@ static lean_object* l_Lean_Meta_Linear_Nat_LinearExpr_toExpr___closed__11;
 static lean_object* l_Lean_Meta_Linear_Nat_LinearCnstr_toExpr___closed__10;
 lean_object* l_Lean_Meta_mkLE(lean_object*, lean_object*, lean_object*, lean_object*, lean_object*, lean_object*, lean_object*);
 static lean_object* l_Lean_Meta_Linear_Nat_ToLinear_State_varMap___default___closed__3;
-uint8_t l___private_Init_Data_Nat_Linear_0__Nat_Linear_beqPolyCnstr____x40_Init_Data_Nat_Linear___hyg_1266_(lean_object*, lean_object*);
+uint8_t l___private_Init_Data_Nat_Linear_0__Nat_Linear_beqPolyCnstr____x40_Init_Data_Nat_Linear___hyg_1453_(lean_object*, lean_object*);
 lean_object* l_Nat_Linear_Poly_toExpr(lean_object*);
 static lean_object* l_Lean_Meta_Linear_Nat_simpCnstr_x3f___lambda__1___closed__4;
 static lean_object* l_Lean_Meta_Linear_Nat_simpCnstr_x3f___lambda__1___closed__1;
@@ -4467,7 +4467,7 @@ x_28 = l_Nat_Linear_PolyCnstr_isValid(x_26);
 if (x_28 == 0)
 {
 uint8_t x_29; 
-x_29 = l___private_Init_Data_Nat_Linear_0__Nat_Linear_beqPolyCnstr____x40_Init_Data_Nat_Linear___hyg_1266_(x_25, x_26);
+x_29 = l___private_Init_Data_Nat_Linear_0__Nat_Linear_beqPolyCnstr____x40_Init_Data_Nat_Linear___hyg_1453_(x_25, x_26);
 lean_dec(x_25);
 if (x_29 == 0)
 {
@@ -4769,7 +4769,7 @@ x_98 = l_Nat_Linear_PolyCnstr_isValid(x_96);
 if (x_98 == 0)
 {
 uint8_t x_99; 
-x_99 = l___private_Init_Data_Nat_Linear_0__Nat_Linear_beqPolyCnstr____x40_Init_Data_Nat_Linear___hyg_1266_(x_95, x_96);
+x_99 = l___private_Init_Data_Nat_Linear_0__Nat_Linear_beqPolyCnstr____x40_Init_Data_Nat_Linear___hyg_1453_(x_95, x_96);
 lean_dec(x_95);
 if (x_99 == 0)
 {
@@ -5065,7 +5065,7 @@ x_160 = l_Nat_Linear_PolyCnstr_isValid(x_158);
 if (x_160 == 0)
 {
 uint8_t x_161; 
-x_161 = l___private_Init_Data_Nat_Linear_0__Nat_Linear_beqPolyCnstr____x40_Init_Data_Nat_Linear___hyg_1266_(x_157, x_158);
+x_161 = l___private_Init_Data_Nat_Linear_0__Nat_Linear_beqPolyCnstr____x40_Init_Data_Nat_Linear___hyg_1453_(x_157, x_158);
 lean_dec(x_157);
 if (x_161 == 0)
 {
@@ -5386,7 +5386,7 @@ x_227 = l_Nat_Linear_PolyCnstr_isValid(x_225);
 if (x_227 == 0)
 {
 uint8_t x_228; 
-x_228 = l___private_Init_Data_Nat_Linear_0__Nat_Linear_beqPolyCnstr____x40_Init_Data_Nat_Linear___hyg_1266_(x_224, x_225);
+x_228 = l___private_Init_Data_Nat_Linear_0__Nat_Linear_beqPolyCnstr____x40_Init_Data_Nat_Linear___hyg_1453_(x_224, x_225);
 lean_dec(x_224);
 if (x_228 == 0)
 {
