stage0/stdlib/Lean/Meta/Tactic/Simp/SimpTheorems.c
@@ -16,6 +16,7 @@ extern "C" {
 LEAN_EXPORT lean_object* l_Lean_Meta_SimpTheorem_getName___boxed(lean_object*);
 LEAN_EXPORT lean_object* l_Array_forInUnsafe_loop___at_Lean_Meta_SimpTheorems_addDeclToUnfold___spec__1___boxed(lean_object*, lean_object*, lean_object*, lean_object*, lean_object*, lean_object*, lean_object*, lean_object*, lean_object*);
 static lean_object* l_Lean_Meta_SimpTheorems_erase___rarg___closed__2;
+static lean_object* l_Lean_Meta_initFn____x40_Lean_Meta_Tactic_Simp_SimpTheorems___hyg_4092____closed__1;
 static lean_object* l_Lean_Meta_mkSimpAttr___lambda__1___closed__2;
 LEAN_EXPORT lean_object* l_Lean_Meta_SimpTheorems_pre___default;
 lean_object* l_Lean_ScopedEnvExtension_modifyState___rarg(lean_object*, lean_object*, lean_object*);
@@ -28,9 +29,9 @@ LEAN_EXPORT lean_object* l_Lean_Meta_SimpTheorems_isLemma___boxed(lean_object*, 
 LEAN_EXPORT lean_object* l_Lean_Meta_SimpTheorems_erase___rarg(lean_object*, lean_object*, lean_object*, lean_object*);
 LEAN_EXPORT lean_object* l_Lean_Meta_SimpTheorems_erase___at_Lean_Meta_mkSimpAttr___spec__2___lambda__1(lean_object*, lean_object*, lean_object*, lean_object*, lean_object*, lean_object*);
 LEAN_EXPORT lean_object* l_Std_PersistentHashMap_insert___at_Lean_Meta_addSimpTheoremEntry___spec__5(lean_object*, lean_object*, lean_object*);
-static lean_object* l_Lean_Meta_initFn____x40_Lean_Meta_Tactic_Simp_SimpTheorems___hyg_3740____closed__3;
+static lean_object* l_Lean_Meta_initFn____x40_Lean_Meta_Tactic_Simp_SimpTheorems___hyg_4092____closed__2;
 LEAN_EXPORT lean_object* l_Lean_Meta_getSimpTheorems(lean_object*, lean_object*, lean_object*);
-static lean_object* l_Lean_Meta_initFn____x40_Lean_Meta_Tactic_Simp_SimpTheorems___hyg_3740____closed__2;
+static lean_object* l___private_Lean_Meta_Tactic_Simp_SimpTheorems_0__Lean_Meta_preprocess_go___lambda__3___closed__7;
 lean_object* l_Lean_stringToMessageData(lean_object*);
 LEAN_EXPORT lean_object* l_Lean_Meta_SimpTheorems_addDeclToUnfold___lambda__1(lean_object*, lean_object*, lean_object*, lean_object*, lean_object*, lean_object*, lean_object*);
 lean_object* lean_mk_empty_array_with_capacity(lean_object*);
@@ -51,10 +52,10 @@ uint64_t lean_uint64_of_nat(lean_object*);
 LEAN_EXPORT lean_object* l_Array_forInUnsafe_loop___at_Lean_Meta_mkSimpAttr___spec__1(lean_object*, uint8_t, uint8_t, lean_object*, lean_object*, size_t, size_t, lean_object*, lean_object*, lean_object*, lean_object*, lean_object*, lean_object*);
 static lean_object* l___private_Lean_Meta_Tactic_Simp_SimpTheorems_0__Lean_Meta_preprocess_go___closed__6;
 LEAN_EXPORT lean_object* l_Lean_Meta_addSimpTheoremEntry_updateLemmaNames(lean_object*, lean_object*);
+lean_object* l_Lean_Meta_mkAppM(lean_object*, lean_object*, lean_object*, lean_object*, lean_object*, lean_object*, lean_object*);
 static lean_object* l_Lean_Meta_SimpTheorems_erase___rarg___closed__1;
 lean_object* lean_array_uset(lean_object*, size_t, lean_object*);
 lean_object* l_Lean_throwError___at___private_Lean_Meta_Basic_0__Lean_Meta_processPostponedStep___spec__1(lean_object*, lean_object*, lean_object*, lean_object*, lean_object*, lean_object*);
-LEAN_EXPORT lean_object* l___private_Lean_Meta_Tactic_Simp_SimpTheorems_0__Lean_Meta_preprocess_go___lambda__5___boxed(lean_object*, lean_object*, lean_object*, lean_object*, lean_object*, lean_object*, lean_object*, lean_object*, lean_object*, lean_object*, lean_object*);
 lean_object* l_Lean_registerSimpleScopedEnvExtension___rarg(lean_object*, lean_object*);
 LEAN_EXPORT lean_object* l___private_Lean_Meta_DiscrTree_0__Lean_Meta_DiscrTree_insertAux___at_Lean_Meta_addSimpTheoremEntry___spec__9(lean_object*, lean_object*, lean_object*, lean_object*);
 lean_object* l_Lean_Meta_forallTelescopeReducing___at_Lean_Meta_getParamNames___spec__2___rarg(lean_object*, lean_object*, lean_object*, lean_object*, lean_object*, lean_object*, lean_object*);
@@ -70,11 +71,11 @@ static lean_object* l_Lean_Meta_SimpTheorem_keys___default___closed__1;
 LEAN_EXPORT uint8_t l_Lean_Meta_instBEqSimpTheorem(lean_object*, lean_object*);
 LEAN_EXPORT lean_object* l_Lean_throwError___at___private_Lean_Meta_Tactic_Simp_SimpTheorems_0__Lean_Meta_mkSimpTheoremCore___spec__1___boxed(lean_object*, lean_object*, lean_object*, lean_object*, lean_object*, lean_object*);
 LEAN_EXPORT lean_object* l_Lean_Meta_SimpTheorem_priority___default;
-static lean_object* l_Lean_Meta_initFn____x40_Lean_Meta_Tactic_Simp_SimpTheorems___hyg_3740____closed__1;
 lean_object* l_Lean_Meta_DiscrTree_whnfDT(lean_object*, uint8_t, lean_object*, lean_object*, lean_object*, lean_object*, lean_object*);
 lean_object* l_id___rarg___boxed(lean_object*);
 lean_object* lean_st_ref_get(lean_object*, lean_object*);
 LEAN_EXPORT uint8_t l_Lean_Meta_SimpTheorems_isDeclToUnfold(lean_object*, lean_object*);
+LEAN_EXPORT lean_object* l___private_Lean_Meta_Tactic_Simp_SimpTheorems_0__Lean_Meta_preprocess_go___lambda__7___boxed(lean_object*, lean_object*, lean_object*, lean_object*, lean_object*, lean_object*, lean_object*, lean_object*, lean_object*, lean_object*, lean_object*);
 LEAN_EXPORT lean_object* l_panic___at_Lean_Meta_addSimpTheoremEntry___spec__15(lean_object*);
 LEAN_EXPORT lean_object* l___private_Lean_Meta_Tactic_Simp_SimpTheorems_0__Lean_Meta_isPerm(lean_object*, lean_object*, lean_object*, lean_object*, lean_object*, lean_object*, lean_object*);
 LEAN_EXPORT lean_object* l_Std_PersistentHashMap_findAtAux___at_Lean_Meta_SimpTheorems_eraseCore___spec__3(lean_object*, lean_object*, lean_object*, lean_object*, lean_object*);
@@ -86,6 +87,7 @@ static lean_object* l_Lean_Meta_mkSimpAttr___lambda__1___closed__8;
 LEAN_EXPORT lean_object* l_Lean_Meta_SimpTheorems_add(lean_object*, lean_object*, lean_object*, uint8_t, uint8_t, lean_object*, lean_object*, lean_object*, lean_object*, lean_object*, lean_object*, lean_object*);
 LEAN_EXPORT lean_object* l_Std_PersistentHashMap_findAtAux___at_Lean_Meta_addSimpTheoremEntry___spec__4___boxed(lean_object*, lean_object*, lean_object*, lean_object*, lean_object*);
 lean_object* l_Lean_Meta_DiscrTree_instInhabitedDiscrTree(lean_object*);
+static lean_object* l___private_Lean_Meta_Tactic_Simp_SimpTheorems_0__Lean_Meta_preprocess_go___lambda__3___closed__5;
 LEAN_EXPORT lean_object* l_Lean_Meta_mkSimpTheorems___boxed(lean_object*, lean_object*, lean_object*, lean_object*, lean_object*, lean_object*, lean_object*, lean_object*, lean_object*, lean_object*, lean_object*);
 LEAN_EXPORT uint8_t l_Lean_Meta_SimpTheorem_perm___default;
 LEAN_EXPORT lean_object* l_Lean_Meta_SimpTheorems_lemmaNames___default;
@@ -102,7 +104,7 @@ LEAN_EXPORT lean_object* l_Lean_Meta_SimpTheorems_addDeclToUnfold___lambda__2(le
 LEAN_EXPORT lean_object* l_Lean_Meta_SimpTheorems_addDeclToUnfold(lean_object*, lean_object*, lean_object*, lean_object*, lean_object*, lean_object*, lean_object*);
 size_t lean_usize_shift_right(size_t, size_t);
 lean_object* l_Lean_ScopedEnvExtension_addScopedEntry___rarg(lean_object*, lean_object*, lean_object*, lean_object*);
-LEAN_EXPORT lean_object* l___private_Lean_Meta_Tactic_Simp_SimpTheorems_0__Lean_Meta_preprocess_go___lambda__4___boxed(lean_object*, lean_object*, lean_object*, lean_object*, lean_object*, lean_object*, lean_object*, lean_object*, lean_object*, lean_object*);
+LEAN_EXPORT lean_object* l___private_Lean_Meta_Tactic_Simp_SimpTheorems_0__Lean_Meta_preprocess_go___lambda__4___boxed(lean_object*, lean_object*, lean_object*, lean_object*, lean_object*, lean_object*, lean_object*, lean_object*, lean_object*);
 lean_object* l_Lean_Expr_appArg_x21(lean_object*);
 static lean_object* l___private_Lean_Meta_Tactic_Simp_SimpTheorems_0__Lean_Meta_preprocess_go___closed__8;
 static lean_object* l___private_Lean_Meta_Tactic_Simp_SimpTheorems_0__Lean_Meta_shouldPreprocess___closed__1;
@@ -118,18 +120,20 @@ static lean_object* l___private_Lean_Meta_Tactic_Simp_SimpTheorems_0__Lean_Meta_
 LEAN_EXPORT lean_object* l_List_forIn_loop___at___private_Lean_Meta_Tactic_Simp_SimpTheorems_0__Lean_Meta_mkSimpTheoremsFromConst___spec__1___boxed(lean_object*, lean_object*, lean_object*, lean_object*, lean_object*, lean_object*, lean_object*, lean_object*, lean_object*, lean_object*, lean_object*, lean_object*, lean_object*);
 LEAN_EXPORT lean_object* l___private_Lean_Meta_Tactic_Simp_SimpTheorems_0__Lean_Meta_mkSimpTheoremsFromConst___boxed(lean_object*, lean_object*, lean_object*, lean_object*, lean_object*, lean_object*, lean_object*, lean_object*, lean_object*);
 LEAN_EXPORT lean_object* l___private_Lean_Meta_Tactic_Simp_SimpTheorems_0__Lean_Meta_preprocess_go___boxed(lean_object*, lean_object*, lean_object*, lean_object*, lean_object*, lean_object*, lean_object*, lean_object*, lean_object*);
+static lean_object* l_Lean_Meta_initFn____x40_Lean_Meta_Tactic_Simp_SimpTheorems___hyg_4092____closed__3;
 LEAN_EXPORT lean_object* l_Lean_Meta_SimpTheorems_erase(lean_object*);
 LEAN_EXPORT lean_object* l_List_mapM___at___private_Lean_Meta_Tactic_Simp_SimpTheorems_0__Lean_Meta_preprocess_go___spec__1___boxed(lean_object*, lean_object*, lean_object*, lean_object*, lean_object*, lean_object*, lean_object*);
 LEAN_EXPORT uint8_t l_Array_contains___at_Lean_Meta_addSimpTheoremEntry___spec__11(lean_object*, lean_object*);
 lean_object* l_Lean_mkAppN(lean_object*, lean_object*);
 size_t lean_uint64_to_usize(uint64_t);
-static lean_object* l_Lean_Meta_initFn____x40_Lean_Meta_Tactic_Simp_SimpTheorems___hyg_3740____closed__5;
 uint8_t l___private_Lean_Meta_DiscrTreeTypes_0__Lean_Meta_DiscrTree_beqKey____x40_Lean_Meta_DiscrTreeTypes___hyg_89_(lean_object*, lean_object*);
 LEAN_EXPORT uint8_t l_Std_PersistentHashMap_contains___at_Lean_Meta_SimpTheorems_erase___spec__1(lean_object*, lean_object*);
 lean_object* l_Lean_getAttrParamOptPrio(lean_object*, lean_object*, lean_object*, lean_object*);
+static lean_object* l___private_Lean_Meta_Tactic_Simp_SimpTheorems_0__Lean_Meta_preprocess_go___lambda__3___closed__12;
 LEAN_EXPORT lean_object* l_Lean_Meta_SimpTheorem_keys___default;
 lean_object* l_Lean_ConstantInfo_levelParams(lean_object*);
 static lean_object* l_Lean_Meta_instInhabitedSimpTheorems___closed__1;
+static lean_object* l_Lean_Meta_initFn____x40_Lean_Meta_Tactic_Simp_SimpTheorems___hyg_4092____closed__5;
 static lean_object* l_Lean_Meta_mkSimpAttr___lambda__1___closed__19;
 lean_object* lean_array_fget(lean_object*, lean_object*);
 lean_object* l_Lean_mkProj(lean_object*, lean_object*, lean_object*);
@@ -145,7 +149,6 @@ static lean_object* l___private_Lean_Meta_Tactic_Simp_SimpTheorems_0__Lean_Meta_
 LEAN_EXPORT lean_object* l_Array_foldlMUnsafe_fold___at_Lean_Meta_SimpTheorems_addConst___spec__1(lean_object*, size_t, size_t, lean_object*);
 lean_object* l___private_Lean_Meta_Basic_0__Lean_Meta_forallMetaTelescopeReducingAux(lean_object*, uint8_t, lean_object*, uint8_t, lean_object*, lean_object*, lean_object*, lean_object*, lean_object*);
 lean_object* lean_st_ref_take(lean_object*, lean_object*);
-static lean_object* l___private_Lean_Meta_Tactic_Simp_SimpTheorems_0__Lean_Meta_mkSimpTheoremsFromConst___closed__1;
 lean_object* l_Lean_ScopedEnvExtension_addLocalEntry___rarg(lean_object*, lean_object*, lean_object*);
 lean_object* lean_nat_sub(lean_object*, lean_object*);
 lean_object* l_Std_PersistentHashMap_insert___at_Lean_NameSSet_insert___spec__2(lean_object*, lean_object*, lean_object*);
@@ -207,6 +210,7 @@ uint8_t l_Lean_Expr_isAppOfArity(lean_object*, lean_object*, lean_object*);
 static lean_object* l_Lean_Meta_SimpTheorems_addDeclToUnfold___lambda__2___closed__1;
 LEAN_EXPORT lean_object* l___private_Lean_Meta_Tactic_Simp_SimpTheorems_0__Lean_Meta_isPerm___lambda__1(lean_object*, lean_object*, lean_object*, lean_object*, lean_object*, lean_object*, lean_object*, lean_object*);
 static lean_object* l_Lean_Meta_SimpTheorem_getValue___closed__4;
+static lean_object* l___private_Lean_Meta_Tactic_Simp_SimpTheorems_0__Lean_Meta_preprocess_go___lambda__3___closed__13;
 lean_object* l_Lean_registerBuiltinAttribute(lean_object*, lean_object*);
 lean_object* l_Lean_Meta_mkEqTrue(lean_object*, lean_object*, lean_object*, lean_object*, lean_object*, lean_object*);
 lean_object* l___private_Init_Util_0__mkPanicMessageWithDecl(lean_object*, lean_object*, lean_object*, lean_object*, lean_object*);
@@ -214,9 +218,11 @@ uint8_t l_Lean_Expr_isConst(lean_object*);
 uint8_t l_Array_isEmpty___rarg(lean_object*);
 static lean_object* l_Lean_Meta_instToFormatSimpTheorem___closed__5;
 LEAN_EXPORT lean_object* l_Lean_Meta_SimpTheorems_isDeclToUnfold___boxed(lean_object*, lean_object*);
+uint8_t l_Lean_Expr_isConstOf(lean_object*, lean_object*);
 LEAN_EXPORT lean_object* l_Lean_Meta_SimpExtension_getTheorems___boxed(lean_object*, lean_object*, lean_object*, lean_object*);
-LEAN_EXPORT lean_object* l_Lean_Meta_initFn____x40_Lean_Meta_Tactic_Simp_SimpTheorems___hyg_3740_(lean_object*);
+LEAN_EXPORT lean_object* l_Lean_Meta_initFn____x40_Lean_Meta_Tactic_Simp_SimpTheorems___hyg_4092_(lean_object*);
 size_t lean_usize_mul(size_t, size_t);
+static lean_object* l___private_Lean_Meta_Tactic_Simp_SimpTheorems_0__Lean_Meta_preprocess_go___lambda__3___closed__9;
 LEAN_EXPORT lean_object* l_Lean_Meta_SimpTheorems_eraseCore(lean_object*, lean_object*);
 uint8_t l_Lean_Expr_isForall(lean_object*);
 LEAN_EXPORT lean_object* l_Array_contains___at_Lean_Meta_addSimpTheoremEntry___spec__11___boxed(lean_object*, lean_object*);
@@ -234,6 +240,7 @@ lean_object* l_Lean_ConstantInfo_type(lean_object*);
 LEAN_EXPORT lean_object* l_Lean_Meta_SimpTheorem_getValue___boxed(lean_object*, lean_object*, lean_object*, lean_object*, lean_object*, lean_object*);
 lean_object* l_instBEqProd___rarg(lean_object*, lean_object*, lean_object*, lean_object*);
 LEAN_EXPORT lean_object* l_Array_binInsertM___at_Lean_Meta_addSimpTheoremEntry___spec__13___boxed(lean_object*, lean_object*, lean_object*, lean_object*, lean_object*, lean_object*, lean_object*);
+static lean_object* l___private_Lean_Meta_Tactic_Simp_SimpTheorems_0__Lean_Meta_preprocess_go___lambda__3___closed__2;
 static lean_object* l___private_Lean_Meta_Tactic_Simp_SimpTheorems_0__Lean_Meta_preprocess_go___lambda__1___closed__1;
 static lean_object* l_Lean_Meta_SimpTheorems_erase___rarg___closed__3;
 LEAN_EXPORT lean_object* l___private_Lean_Meta_Tactic_Simp_SimpTheorems_0__Lean_Meta_preprocess_go___lambda__6___boxed(lean_object*, lean_object*, lean_object*, lean_object*, lean_object*, lean_object*, lean_object*, lean_object*, lean_object*, lean_object*);
@@ -253,6 +260,7 @@ LEAN_EXPORT lean_object* l_Lean_Meta_SimpTheorems_erased___default;
 static lean_object* l___private_Lean_Meta_Tactic_Simp_SimpTheorems_0__Lean_Meta_checkTypeIsProp___closed__2;
 LEAN_EXPORT lean_object* l___private_Lean_Meta_Tactic_Simp_SimpTheorems_0__Lean_Meta_preprocess_go___lambda__1___boxed(lean_object*, lean_object*, lean_object*, lean_object*, lean_object*, lean_object*, lean_object*, lean_object*);
 LEAN_EXPORT lean_object* l_Std_PersistentHashMap_insertAux___at_Lean_Meta_SimpTheorems_registerDeclToUnfoldThms___spec__2(lean_object*, size_t, size_t, lean_object*, lean_object*);
+static lean_object* l___private_Lean_Meta_Tactic_Simp_SimpTheorems_0__Lean_Meta_preprocess_go___lambda__3___closed__4;
 LEAN_EXPORT lean_object* l_Lean_Meta_SimpTheorem_getValue(lean_object*, lean_object*, lean_object*, lean_object*, lean_object*, lean_object*);
 lean_object* l_List_redLength___rarg(lean_object*);
 static lean_object* l_Lean_Meta_mkSimpAttr___lambda__1___closed__27;
@@ -261,11 +269,14 @@ static lean_object* l_Lean_Meta_mkSimpAttr___lambda__1___closed__4;
 lean_object* lean_name_append_after(lean_object*, lean_object*);
 extern lean_object* l_Lean_Meta_DiscrTree_instInhabitedKey;
 static lean_object* l_Lean_Meta_mkSimpAttr___lambda__1___closed__9;
+static lean_object* l___private_Lean_Meta_Tactic_Simp_SimpTheorems_0__Lean_Meta_preprocess_go___lambda__3___closed__8;
 static lean_object* l___private_Lean_Meta_Tactic_Simp_SimpTheorems_0__Lean_Meta_preprocess_go___lambda__1___closed__3;
 lean_object* l_Lean_Meta_whnfR(lean_object*, lean_object*, lean_object*, lean_object*, lean_object*, lean_object*);
 LEAN_EXPORT lean_object* l___private_Lean_Meta_DiscrTree_0__Lean_Meta_DiscrTree_insertAux___at_Lean_Meta_addSimpTheoremEntry___spec__9___boxed(lean_object*, lean_object*, lean_object*, lean_object*);
+static lean_object* l___private_Lean_Meta_Tactic_Simp_SimpTheorems_0__Lean_Meta_preprocess_go___lambda__3___closed__11;
 uint8_t lean_expr_eqv(lean_object*, lean_object*);
 lean_object* l_Lean_Meta_getEqnsFor_x3f(lean_object*, lean_object*, lean_object*, lean_object*, lean_object*, lean_object*);
+LEAN_EXPORT lean_object* l___private_Lean_Meta_Tactic_Simp_SimpTheorems_0__Lean_Meta_preprocess_go___lambda__8(lean_object*, uint8_t, uint8_t, lean_object*, lean_object*, lean_object*, lean_object*, lean_object*, lean_object*, lean_object*);
 LEAN_EXPORT lean_object* l___private_Lean_Meta_Tactic_Simp_SimpTheorems_0__Lean_Meta_preprocess___boxed(lean_object*, lean_object*, lean_object*, lean_object*, lean_object*, lean_object*, lean_object*, lean_object*, lean_object*);
 uint8_t lean_nat_dec_le(lean_object*, lean_object*);
 LEAN_EXPORT lean_object* l_Array_foldlMUnsafe_fold___at_Lean_Meta_SimpTheorems_eraseCore___spec__4___boxed(lean_object*, lean_object*, lean_object*, lean_object*);
@@ -289,12 +300,13 @@ lean_object* l_Lean_Meta_withLocalDecl___at___private_Lean_Meta_SynthInstance_0_
 static lean_object* l___private_Lean_Meta_Tactic_Simp_SimpTheorems_0__Lean_Meta_preprocess_go___lambda__1___closed__2;
 static lean_object* l_Lean_Meta_mkSimpExt___closed__2;
 uint8_t l_Lean_Meta_DiscrTree_Key_lt(lean_object*, lean_object*);
+static lean_object* l___private_Lean_Meta_Tactic_Simp_SimpTheorems_0__Lean_Meta_preprocess_go___lambda__3___closed__1;
 lean_object* l_List_mapTRAux___at_Lean_mkConstWithLevelParams___spec__1(lean_object*, lean_object*);
 LEAN_EXPORT lean_object* l_Array_mapMUnsafe_map___at___private_Lean_Meta_Tactic_Simp_SimpTheorems_0__Lean_Meta_preprocessProof___spec__1___boxed(lean_object*, lean_object*, lean_object*);
-LEAN_EXPORT lean_object* l___private_Lean_Meta_Tactic_Simp_SimpTheorems_0__Lean_Meta_preprocess_go___lambda__3___boxed(lean_object*, lean_object*, lean_object*, lean_object*, lean_object*, lean_object*, lean_object*, lean_object*, lean_object*);
 LEAN_EXPORT lean_object* l_Lean_Meta_instToMessageDataSimpTheorem(lean_object*);
 lean_object* l_Lean_throwError___rarg(lean_object*, lean_object*, lean_object*);
 static lean_object* l___private_Lean_Meta_DiscrTree_0__Lean_Meta_DiscrTree_insertAux___at_Lean_Meta_addSimpTheoremEntry___spec__9___closed__3;
+static lean_object* l___private_Lean_Meta_Tactic_Simp_SimpTheorems_0__Lean_Meta_preprocess_go___lambda__3___closed__3;
 lean_object* lean_st_ref_set(lean_object*, lean_object*, lean_object*);
 LEAN_EXPORT lean_object* l_Lean_Meta_SimpTheorems_add_getName_x3f___boxed(lean_object*, lean_object*, lean_object*, lean_object*, lean_object*, lean_object*, lean_object*);
 uint8_t l_Lean_Expr_isFVar(lean_object*);
@@ -302,10 +314,11 @@ static lean_object* l_Lean_Meta_mkSimpAttr___lambda__1___closed__18;
 static lean_object* l_Lean_Meta_DiscrTree_insertCore___at_Lean_Meta_addSimpTheoremEntry___spec__1___closed__1;
 lean_object* l_Lean_addMessageContextFull___at_Lean_Meta_instAddMessageContextMetaM___spec__1(lean_object*, lean_object*, lean_object*, lean_object*, lean_object*, lean_object*);
 static lean_object* l_Lean_Meta_mkSimpAttr___lambda__1___closed__15;
-LEAN_EXPORT lean_object* l___private_Lean_Meta_Tactic_Simp_SimpTheorems_0__Lean_Meta_preprocess_go___lambda__4(uint8_t, lean_object*, lean_object*, lean_object*, lean_object*, lean_object*, lean_object*, lean_object*, lean_object*, lean_object*);
+LEAN_EXPORT lean_object* l___private_Lean_Meta_Tactic_Simp_SimpTheorems_0__Lean_Meta_preprocess_go___lambda__4(lean_object*, lean_object*, lean_object*, lean_object*, lean_object*, lean_object*, lean_object*, lean_object*, lean_object*);
 static lean_object* l___private_Lean_Meta_Tactic_Simp_SimpTheorems_0__Lean_Meta_checkBadRewrite___closed__3;
 lean_object* l_List_toArrayAux___rarg(lean_object*, lean_object*);
 uint8_t l_Lean_Syntax_isNone(lean_object*);
+static lean_object* l___private_Lean_Meta_Tactic_Simp_SimpTheorems_0__Lean_Meta_preprocess_go___lambda__3___closed__6;
 lean_object* lean_infer_type(lean_object*, lean_object*, lean_object*, lean_object*, lean_object*, lean_object*);
 static lean_object* l_Lean_Meta_mkSimpAttr___lambda__1___closed__5;
 LEAN_EXPORT lean_object* l___private_Lean_Meta_Tactic_Simp_SimpTheorems_0__Lean_Meta_preprocess_go(uint8_t, uint8_t, lean_object*, lean_object*, lean_object*, lean_object*, lean_object*, lean_object*, lean_object*);
@@ -332,6 +345,7 @@ static lean_object* l_Lean_Meta_instToFormatSimpTheorem___closed__2;
 LEAN_EXPORT lean_object* l_Lean_Meta_SimpTheorems_toUnfold___default;
 static lean_object* l___private_Lean_Meta_Tactic_Simp_SimpTheorems_0__Lean_Meta_preprocess_go___lambda__2___closed__1;
 static lean_object* l_Lean_Meta_instToFormatSimpTheorem___closed__1;
+static lean_object* l___private_Lean_Meta_Tactic_Simp_SimpTheorems_0__Lean_Meta_preprocess_go___lambda__3___closed__10;
 extern lean_object* l_Lean_Expr_instBEqExpr;
 static lean_object* l___private_Lean_Meta_Tactic_Simp_SimpTheorems_0__Lean_Meta_preprocess_go___closed__9;
 LEAN_EXPORT lean_object* l_Std_PersistentHashMap_insertAux___at_Lean_Meta_addSimpTheoremEntry___spec__6(lean_object*, size_t, size_t, lean_object*, lean_object*);
@@ -344,7 +358,7 @@ static lean_object* l_Lean_Meta_mkSimpAttr___lambda__1___closed__24;
 lean_object* l_Lean_Expr_instantiateLevelParamsCore_visit___at_Lean_Expr_instantiateLevelParamsArray___spec__1(lean_object*, lean_object*, lean_object*);
 LEAN_EXPORT lean_object* l_Lean_Meta_SimpTheorems_addConst___boxed(lean_object*, lean_object*, lean_object*, lean_object*, lean_object*, lean_object*, lean_object*, lean_object*, lean_object*, lean_object*);
 LEAN_EXPORT uint8_t l_Lean_Meta_SimpTheorem_post___default;
-LEAN_EXPORT lean_object* l___private_Lean_Meta_Tactic_Simp_SimpTheorems_0__Lean_Meta_preprocess_go___lambda__6(lean_object*, uint8_t, uint8_t, lean_object*, lean_object*, lean_object*, lean_object*, lean_object*, lean_object*, lean_object*);
+LEAN_EXPORT lean_object* l___private_Lean_Meta_Tactic_Simp_SimpTheorems_0__Lean_Meta_preprocess_go___lambda__6(uint8_t, lean_object*, lean_object*, lean_object*, lean_object*, lean_object*, lean_object*, lean_object*, lean_object*, lean_object*);
 static lean_object* l_Lean_Meta_DiscrTree_insertCore___at_Lean_Meta_addSimpTheoremEntry___spec__1___closed__3;
 lean_object* l_Lean_Syntax_getArg(lean_object*, lean_object*);
 static lean_object* l_Lean_Meta_instToFormatSimpTheorem___closed__4;
@@ -368,7 +382,6 @@ LEAN_EXPORT lean_object* l___private_Lean_Meta_Tactic_Simp_SimpTheorems_0__Lean_
 static lean_object* l_Lean_Meta_instInhabitedSimpTheorem___closed__3;
 LEAN_EXPORT lean_object* l_Std_PersistentHashMap_insertAtCollisionNodeAux___at_Lean_Meta_SimpTheorems_registerDeclToUnfoldThms___spec__4(lean_object*, lean_object*, lean_object*, lean_object*);
 LEAN_EXPORT lean_object* l_Lean_Meta_addSimpTheorem___boxed(lean_object*, lean_object*, lean_object*, lean_object*, lean_object*, lean_object*, lean_object*, lean_object*, lean_object*, lean_object*, lean_object*);
-static lean_object* l_Lean_Meta_initFn____x40_Lean_Meta_Tactic_Simp_SimpTheorems___hyg_3740____closed__4;
 lean_object* lean_usize_to_nat(size_t);
 lean_object* l___private_Lean_Meta_Basic_0__Lean_Meta_withLetDeclImp___rarg(lean_object*, lean_object*, lean_object*, lean_object*, lean_object*, lean_object*, lean_object*, lean_object*, lean_object*);
 LEAN_EXPORT lean_object* l___private_Lean_Meta_Tactic_Simp_SimpTheorems_0__Lean_Meta_preprocess_go___lambda__3(lean_object*, lean_object*, lean_object*, lean_object*, lean_object*, lean_object*, lean_object*, lean_object*, lean_object*);
@@ -377,7 +390,7 @@ lean_object* l_Lean_Meta_isProp(lean_object*, lean_object*, lean_object*, lean_o
 LEAN_EXPORT lean_object* l___private_Lean_Meta_Tactic_Simp_SimpTheorems_0__Lean_Meta_preprocess(lean_object*, lean_object*, uint8_t, uint8_t, lean_object*, lean_object*, lean_object*, lean_object*, lean_object*);
 LEAN_EXPORT lean_object* l___private_Lean_Meta_Tactic_Simp_SimpTheorems_0__Lean_Meta_mkSimpTheoremCore(lean_object*, lean_object*, lean_object*, uint8_t, lean_object*, lean_object*, lean_object*, lean_object*, lean_object*, lean_object*, lean_object*);
 lean_object* l_Lean_indentExpr(lean_object*);
-LEAN_EXPORT lean_object* l___private_Lean_Meta_Tactic_Simp_SimpTheorems_0__Lean_Meta_preprocess_go___lambda__5(uint8_t, lean_object*, lean_object*, lean_object*, lean_object*, lean_object*, lean_object*, lean_object*, lean_object*, lean_object*, lean_object*);
+LEAN_EXPORT lean_object* l___private_Lean_Meta_Tactic_Simp_SimpTheorems_0__Lean_Meta_preprocess_go___lambda__5(lean_object*, lean_object*, lean_object*, lean_object*, lean_object*, lean_object*, lean_object*, lean_object*, lean_object*);
 LEAN_EXPORT lean_object* l_Lean_Meta_addSimpTheoremEntry(lean_object*, lean_object*);
 static lean_object* l_Lean_Meta_mkSimpAttr___lambda__1___closed__22;
 LEAN_EXPORT lean_object* l_Lean_ScopedEnvExtension_add___at_Lean_Meta_addSimpTheorem___spec__1(lean_object*, lean_object*, uint8_t, lean_object*, lean_object*, lean_object*, lean_object*, lean_object*);
@@ -389,6 +402,7 @@ LEAN_EXPORT lean_object* l_Std_PersistentHashMap_insertAux_traverse___at_Lean_Me
 lean_object* l_Lean_Expr_constName_x21(lean_object*);
 lean_object* l_Array_insertAt___rarg(lean_object*, lean_object*, lean_object*);
 LEAN_EXPORT lean_object* l_Lean_Meta_mkSimpTheorems(lean_object*, lean_object*, uint8_t, uint8_t, lean_object*, lean_object*, lean_object*, lean_object*, lean_object*, lean_object*, lean_object*);
+LEAN_EXPORT lean_object* l___private_Lean_Meta_Tactic_Simp_SimpTheorems_0__Lean_Meta_preprocess_go___lambda__8___boxed(lean_object*, lean_object*, lean_object*, lean_object*, lean_object*, lean_object*, lean_object*, lean_object*, lean_object*, lean_object*);
 LEAN_EXPORT lean_object* l_Lean_Meta_mkSimpAttr(lean_object*, lean_object*, lean_object*, lean_object*);
 LEAN_EXPORT lean_object* l_Std_PersistentHashMap_insertAux_traverse___at_Lean_Meta_SimpTheorems_registerDeclToUnfoldThms___spec__3___boxed(lean_object*, lean_object*, lean_object*, lean_object*, lean_object*, lean_object*);
 static lean_object* l___private_Lean_Meta_Tactic_Simp_SimpTheorems_0__Lean_Meta_preprocess_go___closed__11;
@@ -415,9 +429,11 @@ LEAN_EXPORT lean_object* l_Array_forInUnsafe_loop___at_Lean_Meta_addSimpTheorem_
 lean_object* l_Lean_Meta_DiscrTree_empty(lean_object*);
 LEAN_EXPORT lean_object* l_Lean_Meta_SimpTheorem_levelParams___default;
 lean_object* l_Std_PersistentHashMap_mkCollisionNode___rarg(lean_object*, lean_object*, lean_object*, lean_object*);
+static lean_object* l_Lean_Meta_initFn____x40_Lean_Meta_Tactic_Simp_SimpTheorems___hyg_4092____closed__4;
 LEAN_EXPORT lean_object* l_List_forIn_loop___at___private_Lean_Meta_Tactic_Simp_SimpTheorems_0__Lean_Meta_mkSimpTheoremsFromConst___spec__1(lean_object*, uint8_t, lean_object*, lean_object*, lean_object*, lean_object*, lean_object*, lean_object*, lean_object*, lean_object*, lean_object*, lean_object*, lean_object*);
 static uint64_t l_Lean_Meta_instInhabitedSimpTheorem___closed__1;
 uint8_t lean_nat_dec_lt(lean_object*, lean_object*);
+LEAN_EXPORT lean_object* l___private_Lean_Meta_Tactic_Simp_SimpTheorems_0__Lean_Meta_preprocess_go___lambda__7(uint8_t, lean_object*, lean_object*, lean_object*, lean_object*, lean_object*, lean_object*, lean_object*, lean_object*, lean_object*, lean_object*);
 lean_object* l_Lean_Meta_getFVarLocalDecl(lean_object*, lean_object*, lean_object*, lean_object*, lean_object*, lean_object*);
 static lean_object* l_Lean_Meta_mkSimpAttr___lambda__1___closed__3;
 static lean_object* _init_l_Lean_Meta_SimpTheorem_keys___default___closed__1() {
@@ -5752,7 +5768,393 @@ return x_31;
 }
 }
 }
+static lean_object* _init_l___private_Lean_Meta_Tactic_Simp_SimpTheorems_0__Lean_Meta_preprocess_go___lambda__3___closed__1() {
+_start:
+{
+lean_object* x_1; 
+x_1 = lean_mk_string("Bool");
+return x_1;
+}
+}
+static lean_object* _init_l___private_Lean_Meta_Tactic_Simp_SimpTheorems_0__Lean_Meta_preprocess_go___lambda__3___closed__2() {
+_start:
+{
+lean_object* x_1; lean_object* x_2; lean_object* x_3; 
+x_1 = lean_box(0);
+x_2 = l___private_Lean_Meta_Tactic_Simp_SimpTheorems_0__Lean_Meta_preprocess_go___lambda__3___closed__1;
+x_3 = lean_name_mk_string(x_1, x_2);
+return x_3;
+}
+}
+static lean_object* _init_l___private_Lean_Meta_Tactic_Simp_SimpTheorems_0__Lean_Meta_preprocess_go___lambda__3___closed__3() {
+_start:
+{
+lean_object* x_1; 
+x_1 = lean_mk_string("true");
+return x_1;
+}
+}
+static lean_object* _init_l___private_Lean_Meta_Tactic_Simp_SimpTheorems_0__Lean_Meta_preprocess_go___lambda__3___closed__4() {
+_start:
+{
+lean_object* x_1; lean_object* x_2; lean_object* x_3; 
+x_1 = l___private_Lean_Meta_Tactic_Simp_SimpTheorems_0__Lean_Meta_preprocess_go___lambda__3___closed__2;
+x_2 = l___private_Lean_Meta_Tactic_Simp_SimpTheorems_0__Lean_Meta_preprocess_go___lambda__3___closed__3;
+x_3 = lean_name_mk_string(x_1, x_2);
+return x_3;
+}
+}
+static lean_object* _init_l___private_Lean_Meta_Tactic_Simp_SimpTheorems_0__Lean_Meta_preprocess_go___lambda__3___closed__5() {
+_start:
+{
+lean_object* x_1; 
+x_1 = lean_mk_string("false");
+return x_1;
+}
+}
+static lean_object* _init_l___private_Lean_Meta_Tactic_Simp_SimpTheorems_0__Lean_Meta_preprocess_go___lambda__3___closed__6() {
+_start:
+{
+lean_object* x_1; lean_object* x_2; lean_object* x_3; 
+x_1 = l___private_Lean_Meta_Tactic_Simp_SimpTheorems_0__Lean_Meta_preprocess_go___lambda__3___closed__2;
+x_2 = l___private_Lean_Meta_Tactic_Simp_SimpTheorems_0__Lean_Meta_preprocess_go___lambda__3___closed__5;
+x_3 = lean_name_mk_string(x_1, x_2);
+return x_3;
+}
+}
+static lean_object* _init_l___private_Lean_Meta_Tactic_Simp_SimpTheorems_0__Lean_Meta_preprocess_go___lambda__3___closed__7() {
+_start:
+{
+lean_object* x_1; 
+x_1 = lean_mk_string("of_not_eq_false");
+return x_1;
+}
+}
+static lean_object* _init_l___private_Lean_Meta_Tactic_Simp_SimpTheorems_0__Lean_Meta_preprocess_go___lambda__3___closed__8() {
+_start:
+{
+lean_object* x_1; lean_object* x_2; lean_object* x_3; 
+x_1 = l___private_Lean_Meta_Tactic_Simp_SimpTheorems_0__Lean_Meta_preprocess_go___lambda__3___closed__2;
+x_2 = l___private_Lean_Meta_Tactic_Simp_SimpTheorems_0__Lean_Meta_preprocess_go___lambda__3___closed__7;
+x_3 = lean_name_mk_string(x_1, x_2);
+return x_3;
+}
+}
+static lean_object* _init_l___private_Lean_Meta_Tactic_Simp_SimpTheorems_0__Lean_Meta_preprocess_go___lambda__3___closed__9() {
+_start:
+{
+lean_object* x_1; lean_object* x_2; 
+x_1 = lean_unsigned_to_nat(1u);
+x_2 = lean_mk_empty_array_with_capacity(x_1);
+return x_2;
+}
+}
+static lean_object* _init_l___private_Lean_Meta_Tactic_Simp_SimpTheorems_0__Lean_Meta_preprocess_go___lambda__3___closed__10() {
+_start:
+{
+lean_object* x_1; lean_object* x_2; lean_object* x_3; 
+x_1 = lean_box(0);
+x_2 = l___private_Lean_Meta_Tactic_Simp_SimpTheorems_0__Lean_Meta_preprocess_go___lambda__3___closed__4;
+x_3 = l_Lean_mkConst(x_2, x_1);
+return x_3;
+}
+}
+static lean_object* _init_l___private_Lean_Meta_Tactic_Simp_SimpTheorems_0__Lean_Meta_preprocess_go___lambda__3___closed__11() {
+_start:
+{
+lean_object* x_1; 
+x_1 = lean_mk_string("of_not_eq_true");
+return x_1;
+}
+}
+static lean_object* _init_l___private_Lean_Meta_Tactic_Simp_SimpTheorems_0__Lean_Meta_preprocess_go___lambda__3___closed__12() {
+_start:
+{
+lean_object* x_1; lean_object* x_2; lean_object* x_3; 
+x_1 = l___private_Lean_Meta_Tactic_Simp_SimpTheorems_0__Lean_Meta_preprocess_go___lambda__3___closed__2;
+x_2 = l___private_Lean_Meta_Tactic_Simp_SimpTheorems_0__Lean_Meta_preprocess_go___lambda__3___closed__11;
+x_3 = lean_name_mk_string(x_1, x_2);
+return x_3;
+}
+}
+static lean_object* _init_l___private_Lean_Meta_Tactic_Simp_SimpTheorems_0__Lean_Meta_preprocess_go___lambda__3___closed__13() {
+_start:
+{
+lean_object* x_1; lean_object* x_2; lean_object* x_3; 
+x_1 = lean_box(0);
+x_2 = l___private_Lean_Meta_Tactic_Simp_SimpTheorems_0__Lean_Meta_preprocess_go___lambda__3___closed__6;
+x_3 = l_Lean_mkConst(x_2, x_1);
+return x_3;
+}
+}
 LEAN_EXPORT lean_object* l___private_Lean_Meta_Tactic_Simp_SimpTheorems_0__Lean_Meta_preprocess_go___lambda__3(lean_object* x_1, lean_object* x_2, lean_object* x_3, lean_object* x_4, lean_object* x_5, lean_object* x_6, lean_object* x_7, lean_object* x_8, lean_object* x_9) {
+_start:
+{
+lean_object* x_10; uint8_t x_11; 
+lean_dec(x_4);
+x_10 = lean_unsigned_to_nat(3u);
+x_11 = l_Lean_Expr_isAppOfArity(x_1, x_3, x_10);
+lean_dec(x_3);
+if (x_11 == 0)
+{
+lean_object* x_12; lean_object* x_13; 
+x_12 = lean_box(0);
+x_13 = l___private_Lean_Meta_Tactic_Simp_SimpTheorems_0__Lean_Meta_preprocess_go___lambda__2(x_1, x_2, x_12, x_5, x_6, x_7, x_8, x_9);
+return x_13;
+}
+else
+{
+lean_object* x_14; lean_object* x_15; lean_object* x_16; lean_object* x_17; uint8_t x_18; 
+x_14 = l_Lean_Expr_appFn_x21(x_1);
+x_15 = l_Lean_Expr_appArg_x21(x_14);
+lean_dec(x_14);
+x_16 = l_Lean_Expr_appArg_x21(x_1);
+x_17 = l___private_Lean_Meta_Tactic_Simp_SimpTheorems_0__Lean_Meta_preprocess_go___lambda__3___closed__4;
+x_18 = l_Lean_Expr_isConstOf(x_16, x_17);
+if (x_18 == 0)
+{
+lean_object* x_19; uint8_t x_20; 
+x_19 = l___private_Lean_Meta_Tactic_Simp_SimpTheorems_0__Lean_Meta_preprocess_go___lambda__3___closed__6;
+x_20 = l_Lean_Expr_isConstOf(x_16, x_19);
+lean_dec(x_16);
+if (x_20 == 0)
+{
+lean_object* x_21; lean_object* x_22; 
+lean_dec(x_15);
+x_21 = lean_box(0);
+x_22 = l___private_Lean_Meta_Tactic_Simp_SimpTheorems_0__Lean_Meta_preprocess_go___lambda__2(x_1, x_2, x_21, x_5, x_6, x_7, x_8, x_9);
+return x_22;
+}
+else
+{
+lean_object* x_23; lean_object* x_24; lean_object* x_25; lean_object* x_26; 
+lean_dec(x_1);
+x_23 = l___private_Lean_Meta_Tactic_Simp_SimpTheorems_0__Lean_Meta_preprocess_go___lambda__3___closed__9;
+x_24 = lean_array_push(x_23, x_2);
+x_25 = l___private_Lean_Meta_Tactic_Simp_SimpTheorems_0__Lean_Meta_preprocess_go___lambda__3___closed__8;
+lean_inc(x_8);
+lean_inc(x_7);
+lean_inc(x_6);
+lean_inc(x_5);
+x_26 = l_Lean_Meta_mkAppM(x_25, x_24, x_5, x_6, x_7, x_8, x_9);
+if (lean_obj_tag(x_26) == 0)
+{
+lean_object* x_27; lean_object* x_28; lean_object* x_29; lean_object* x_30; lean_object* x_31; 
+x_27 = lean_ctor_get(x_26, 0);
+lean_inc(x_27);
+x_28 = lean_ctor_get(x_26, 1);
+lean_inc(x_28);
+lean_dec(x_26);
+x_29 = lean_box(0);
+x_30 = l___private_Lean_Meta_Tactic_Simp_SimpTheorems_0__Lean_Meta_preprocess_go___lambda__3___closed__10;
+x_31 = l_Lean_Meta_mkEq(x_15, x_30, x_5, x_6, x_7, x_8, x_28);
+if (lean_obj_tag(x_31) == 0)
+{
+uint8_t x_32; 
+x_32 = !lean_is_exclusive(x_31);
+if (x_32 == 0)
+{
+lean_object* x_33; lean_object* x_34; lean_object* x_35; 
+x_33 = lean_ctor_get(x_31, 0);
+x_34 = lean_alloc_ctor(0, 2, 0);
+lean_ctor_set(x_34, 0, x_27);
+lean_ctor_set(x_34, 1, x_33);
+x_35 = lean_alloc_ctor(1, 2, 0);
+lean_ctor_set(x_35, 0, x_34);
+lean_ctor_set(x_35, 1, x_29);
+lean_ctor_set(x_31, 0, x_35);
+return x_31;
+}
+else
+{
+lean_object* x_36; lean_object* x_37; lean_object* x_38; lean_object* x_39; lean_object* x_40; 
+x_36 = lean_ctor_get(x_31, 0);
+x_37 = lean_ctor_get(x_31, 1);
+lean_inc(x_37);
+lean_inc(x_36);
+lean_dec(x_31);
+x_38 = lean_alloc_ctor(0, 2, 0);
+lean_ctor_set(x_38, 0, x_27);
+lean_ctor_set(x_38, 1, x_36);
+x_39 = lean_alloc_ctor(1, 2, 0);
+lean_ctor_set(x_39, 0, x_38);
+lean_ctor_set(x_39, 1, x_29);
+x_40 = lean_alloc_ctor(0, 2, 0);
+lean_ctor_set(x_40, 0, x_39);
+lean_ctor_set(x_40, 1, x_37);
+return x_40;
+}
+}
+else
+{
+uint8_t x_41; 
+lean_dec(x_27);
+x_41 = !lean_is_exclusive(x_31);
+if (x_41 == 0)
+{
+return x_31;
+}
+else
+{
+lean_object* x_42; lean_object* x_43; lean_object* x_44; 
+x_42 = lean_ctor_get(x_31, 0);
+x_43 = lean_ctor_get(x_31, 1);
+lean_inc(x_43);
+lean_inc(x_42);
+lean_dec(x_31);
+x_44 = lean_alloc_ctor(1, 2, 0);
+lean_ctor_set(x_44, 0, x_42);
+lean_ctor_set(x_44, 1, x_43);
+return x_44;
+}
+}
+}
+else
+{
+uint8_t x_45; 
+lean_dec(x_15);
+lean_dec(x_8);
+lean_dec(x_7);
+lean_dec(x_6);
+lean_dec(x_5);
+x_45 = !lean_is_exclusive(x_26);
+if (x_45 == 0)
+{
+return x_26;
+}
+else
+{
+lean_object* x_46; lean_object* x_47; lean_object* x_48; 
+x_46 = lean_ctor_get(x_26, 0);
+x_47 = lean_ctor_get(x_26, 1);
+lean_inc(x_47);
+lean_inc(x_46);
+lean_dec(x_26);
+x_48 = lean_alloc_ctor(1, 2, 0);
+lean_ctor_set(x_48, 0, x_46);
+lean_ctor_set(x_48, 1, x_47);
+return x_48;
+}
+}
+}
+}
+else
+{
+lean_object* x_49; lean_object* x_50; lean_object* x_51; lean_object* x_52; 
+lean_dec(x_16);
+lean_dec(x_1);
+x_49 = l___private_Lean_Meta_Tactic_Simp_SimpTheorems_0__Lean_Meta_preprocess_go___lambda__3___closed__9;
+x_50 = lean_array_push(x_49, x_2);
+x_51 = l___private_Lean_Meta_Tactic_Simp_SimpTheorems_0__Lean_Meta_preprocess_go___lambda__3___closed__12;
+lean_inc(x_8);
+lean_inc(x_7);
+lean_inc(x_6);
+lean_inc(x_5);
+x_52 = l_Lean_Meta_mkAppM(x_51, x_50, x_5, x_6, x_7, x_8, x_9);
+if (lean_obj_tag(x_52) == 0)
+{
+lean_object* x_53; lean_object* x_54; lean_object* x_55; lean_object* x_56; lean_object* x_57; 
+x_53 = lean_ctor_get(x_52, 0);
+lean_inc(x_53);
+x_54 = lean_ctor_get(x_52, 1);
+lean_inc(x_54);
+lean_dec(x_52);
+x_55 = lean_box(0);
+x_56 = l___private_Lean_Meta_Tactic_Simp_SimpTheorems_0__Lean_Meta_preprocess_go___lambda__3___closed__13;
+x_57 = l_Lean_Meta_mkEq(x_15, x_56, x_5, x_6, x_7, x_8, x_54);
+if (lean_obj_tag(x_57) == 0)
+{
+uint8_t x_58; 
+x_58 = !lean_is_exclusive(x_57);
+if (x_58 == 0)
+{
+lean_object* x_59; lean_object* x_60; lean_object* x_61; 
+x_59 = lean_ctor_get(x_57, 0);
+x_60 = lean_alloc_ctor(0, 2, 0);
+lean_ctor_set(x_60, 0, x_53);
+lean_ctor_set(x_60, 1, x_59);
+x_61 = lean_alloc_ctor(1, 2, 0);
+lean_ctor_set(x_61, 0, x_60);
+lean_ctor_set(x_61, 1, x_55);
+lean_ctor_set(x_57, 0, x_61);
+return x_57;
+}
+else
+{
+lean_object* x_62; lean_object* x_63; lean_object* x_64; lean_object* x_65; lean_object* x_66; 
+x_62 = lean_ctor_get(x_57, 0);
+x_63 = lean_ctor_get(x_57, 1);
+lean_inc(x_63);
+lean_inc(x_62);
+lean_dec(x_57);
+x_64 = lean_alloc_ctor(0, 2, 0);
+lean_ctor_set(x_64, 0, x_53);
+lean_ctor_set(x_64, 1, x_62);
+x_65 = lean_alloc_ctor(1, 2, 0);
+lean_ctor_set(x_65, 0, x_64);
+lean_ctor_set(x_65, 1, x_55);
+x_66 = lean_alloc_ctor(0, 2, 0);
+lean_ctor_set(x_66, 0, x_65);
+lean_ctor_set(x_66, 1, x_63);
+return x_66;
+}
+}
+else
+{
+uint8_t x_67; 
+lean_dec(x_53);
+x_67 = !lean_is_exclusive(x_57);
+if (x_67 == 0)
+{
+return x_57;
+}
+else
+{
+lean_object* x_68; lean_object* x_69; lean_object* x_70; 
+x_68 = lean_ctor_get(x_57, 0);
+x_69 = lean_ctor_get(x_57, 1);
+lean_inc(x_69);
+lean_inc(x_68);
+lean_dec(x_57);
+x_70 = lean_alloc_ctor(1, 2, 0);
+lean_ctor_set(x_70, 0, x_68);
+lean_ctor_set(x_70, 1, x_69);
+return x_70;
+}
+}
+}
+else
+{
+uint8_t x_71; 
+lean_dec(x_15);
+lean_dec(x_8);
+lean_dec(x_7);
+lean_dec(x_6);
+lean_dec(x_5);
+x_71 = !lean_is_exclusive(x_52);
+if (x_71 == 0)
+{
+return x_52;
+}
+else
+{
+lean_object* x_72; lean_object* x_73; lean_object* x_74; 
+x_72 = lean_ctor_get(x_52, 0);
+x_73 = lean_ctor_get(x_52, 1);
+lean_inc(x_73);
+lean_inc(x_72);
+lean_dec(x_52);
+x_74 = lean_alloc_ctor(1, 2, 0);
+lean_ctor_set(x_74, 0, x_72);
+lean_ctor_set(x_74, 1, x_73);
+return x_74;
+}
+}
+}
+}
+}
+}
+LEAN_EXPORT lean_object* l___private_Lean_Meta_Tactic_Simp_SimpTheorems_0__Lean_Meta_preprocess_go___lambda__4(lean_object* x_1, lean_object* x_2, lean_object* x_3, lean_object* x_4, lean_object* x_5, lean_object* x_6, lean_object* x_7, lean_object* x_8, lean_object* x_9) {
 _start:
 {
 lean_object* x_10; 
@@ -5903,7 +6305,253 @@ return x_39;
 }
 }
 }
-LEAN_EXPORT lean_object* l___private_Lean_Meta_Tactic_Simp_SimpTheorems_0__Lean_Meta_preprocess_go___lambda__4(uint8_t x_1, lean_object* x_2, lean_object* x_3, lean_object* x_4, lean_object* x_5, lean_object* x_6, lean_object* x_7, lean_object* x_8, lean_object* x_9, lean_object* x_10) {
+LEAN_EXPORT lean_object* l___private_Lean_Meta_Tactic_Simp_SimpTheorems_0__Lean_Meta_preprocess_go___lambda__5(lean_object* x_1, lean_object* x_2, lean_object* x_3, lean_object* x_4, lean_object* x_5, lean_object* x_6, lean_object* x_7, lean_object* x_8, lean_object* x_9) {
+_start:
+{
+lean_object* x_10; uint8_t x_11; 
+lean_dec(x_4);
+x_10 = l___private_Lean_Meta_Tactic_Simp_SimpTheorems_0__Lean_Meta_preprocess_go___lambda__3___closed__4;
+x_11 = l_Lean_Expr_isConstOf(x_2, x_10);
+if (x_11 == 0)
+{
+lean_object* x_12; uint8_t x_13; 
+x_12 = l___private_Lean_Meta_Tactic_Simp_SimpTheorems_0__Lean_Meta_preprocess_go___lambda__3___closed__6;
+x_13 = l_Lean_Expr_isConstOf(x_2, x_12);
+if (x_13 == 0)
+{
+lean_object* x_14; lean_object* x_15; 
+x_14 = lean_box(0);
+x_15 = l___private_Lean_Meta_Tactic_Simp_SimpTheorems_0__Lean_Meta_preprocess_go___lambda__4(x_1, x_2, x_3, x_14, x_5, x_6, x_7, x_8, x_9);
+return x_15;
+}
+else
+{
+lean_object* x_16; lean_object* x_17; lean_object* x_18; lean_object* x_19; 
+lean_dec(x_2);
+x_16 = l___private_Lean_Meta_Tactic_Simp_SimpTheorems_0__Lean_Meta_preprocess_go___lambda__3___closed__9;
+x_17 = lean_array_push(x_16, x_3);
+x_18 = l___private_Lean_Meta_Tactic_Simp_SimpTheorems_0__Lean_Meta_preprocess_go___lambda__3___closed__8;
+lean_inc(x_8);
+lean_inc(x_7);
+lean_inc(x_6);
+lean_inc(x_5);
+x_19 = l_Lean_Meta_mkAppM(x_18, x_17, x_5, x_6, x_7, x_8, x_9);
+if (lean_obj_tag(x_19) == 0)
+{
+lean_object* x_20; lean_object* x_21; lean_object* x_22; lean_object* x_23; lean_object* x_24; 
+x_20 = lean_ctor_get(x_19, 0);
+lean_inc(x_20);
+x_21 = lean_ctor_get(x_19, 1);
+lean_inc(x_21);
+lean_dec(x_19);
+x_22 = lean_box(0);
+x_23 = l___private_Lean_Meta_Tactic_Simp_SimpTheorems_0__Lean_Meta_preprocess_go___lambda__3___closed__10;
+x_24 = l_Lean_Meta_mkEq(x_1, x_23, x_5, x_6, x_7, x_8, x_21);
+if (lean_obj_tag(x_24) == 0)
+{
+uint8_t x_25; 
+x_25 = !lean_is_exclusive(x_24);
+if (x_25 == 0)
+{
+lean_object* x_26; lean_object* x_27; lean_object* x_28; 
+x_26 = lean_ctor_get(x_24, 0);
+x_27 = lean_alloc_ctor(0, 2, 0);
+lean_ctor_set(x_27, 0, x_20);
+lean_ctor_set(x_27, 1, x_26);
+x_28 = lean_alloc_ctor(1, 2, 0);
+lean_ctor_set(x_28, 0, x_27);
+lean_ctor_set(x_28, 1, x_22);
+lean_ctor_set(x_24, 0, x_28);
+return x_24;
+}
+else
+{
+lean_object* x_29; lean_object* x_30; lean_object* x_31; lean_object* x_32; lean_object* x_33; 
+x_29 = lean_ctor_get(x_24, 0);
+x_30 = lean_ctor_get(x_24, 1);
+lean_inc(x_30);
+lean_inc(x_29);
+lean_dec(x_24);
+x_31 = lean_alloc_ctor(0, 2, 0);
+lean_ctor_set(x_31, 0, x_20);
+lean_ctor_set(x_31, 1, x_29);
+x_32 = lean_alloc_ctor(1, 2, 0);
+lean_ctor_set(x_32, 0, x_31);
+lean_ctor_set(x_32, 1, x_22);
+x_33 = lean_alloc_ctor(0, 2, 0);
+lean_ctor_set(x_33, 0, x_32);
+lean_ctor_set(x_33, 1, x_30);
+return x_33;
+}
+}
+else
+{
+uint8_t x_34; 
+lean_dec(x_20);
+x_34 = !lean_is_exclusive(x_24);
+if (x_34 == 0)
+{
+return x_24;
+}
+else
+{
+lean_object* x_35; lean_object* x_36; lean_object* x_37; 
+x_35 = lean_ctor_get(x_24, 0);
+x_36 = lean_ctor_get(x_24, 1);
+lean_inc(x_36);
+lean_inc(x_35);
+lean_dec(x_24);
+x_37 = lean_alloc_ctor(1, 2, 0);
+lean_ctor_set(x_37, 0, x_35);
+lean_ctor_set(x_37, 1, x_36);
+return x_37;
+}
+}
+}
+else
+{
+uint8_t x_38; 
+lean_dec(x_8);
+lean_dec(x_7);
+lean_dec(x_6);
+lean_dec(x_5);
+lean_dec(x_1);
+x_38 = !lean_is_exclusive(x_19);
+if (x_38 == 0)
+{
+return x_19;
+}
+else
+{
+lean_object* x_39; lean_object* x_40; lean_object* x_41; 
+x_39 = lean_ctor_get(x_19, 0);
+x_40 = lean_ctor_get(x_19, 1);
+lean_inc(x_40);
+lean_inc(x_39);
+lean_dec(x_19);
+x_41 = lean_alloc_ctor(1, 2, 0);
+lean_ctor_set(x_41, 0, x_39);
+lean_ctor_set(x_41, 1, x_40);
+return x_41;
+}
+}
+}
+}
+else
+{
+lean_object* x_42; lean_object* x_43; lean_object* x_44; lean_object* x_45; 
+lean_dec(x_2);
+x_42 = l___private_Lean_Meta_Tactic_Simp_SimpTheorems_0__Lean_Meta_preprocess_go___lambda__3___closed__9;
+x_43 = lean_array_push(x_42, x_3);
+x_44 = l___private_Lean_Meta_Tactic_Simp_SimpTheorems_0__Lean_Meta_preprocess_go___lambda__3___closed__12;
+lean_inc(x_8);
+lean_inc(x_7);
+lean_inc(x_6);
+lean_inc(x_5);
+x_45 = l_Lean_Meta_mkAppM(x_44, x_43, x_5, x_6, x_7, x_8, x_9);
+if (lean_obj_tag(x_45) == 0)
+{
+lean_object* x_46; lean_object* x_47; lean_object* x_48; lean_object* x_49; lean_object* x_50; 
+x_46 = lean_ctor_get(x_45, 0);
+lean_inc(x_46);
+x_47 = lean_ctor_get(x_45, 1);
+lean_inc(x_47);
+lean_dec(x_45);
+x_48 = lean_box(0);
+x_49 = l___private_Lean_Meta_Tactic_Simp_SimpTheorems_0__Lean_Meta_preprocess_go___lambda__3___closed__13;
+x_50 = l_Lean_Meta_mkEq(x_1, x_49, x_5, x_6, x_7, x_8, x_47);
+if (lean_obj_tag(x_50) == 0)
+{
+uint8_t x_51; 
+x_51 = !lean_is_exclusive(x_50);
+if (x_51 == 0)
+{
+lean_object* x_52; lean_object* x_53; lean_object* x_54; 
+x_52 = lean_ctor_get(x_50, 0);
+x_53 = lean_alloc_ctor(0, 2, 0);
+lean_ctor_set(x_53, 0, x_46);
+lean_ctor_set(x_53, 1, x_52);
+x_54 = lean_alloc_ctor(1, 2, 0);
+lean_ctor_set(x_54, 0, x_53);
+lean_ctor_set(x_54, 1, x_48);
+lean_ctor_set(x_50, 0, x_54);
+return x_50;
+}
+else
+{
+lean_object* x_55; lean_object* x_56; lean_object* x_57; lean_object* x_58; lean_object* x_59; 
+x_55 = lean_ctor_get(x_50, 0);
+x_56 = lean_ctor_get(x_50, 1);
+lean_inc(x_56);
+lean_inc(x_55);
+lean_dec(x_50);
+x_57 = lean_alloc_ctor(0, 2, 0);
+lean_ctor_set(x_57, 0, x_46);
+lean_ctor_set(x_57, 1, x_55);
+x_58 = lean_alloc_ctor(1, 2, 0);
+lean_ctor_set(x_58, 0, x_57);
+lean_ctor_set(x_58, 1, x_48);
+x_59 = lean_alloc_ctor(0, 2, 0);
+lean_ctor_set(x_59, 0, x_58);
+lean_ctor_set(x_59, 1, x_56);
+return x_59;
+}
+}
+else
+{
+uint8_t x_60; 
+lean_dec(x_46);
+x_60 = !lean_is_exclusive(x_50);
+if (x_60 == 0)
+{
+return x_50;
+}
+else
+{
+lean_object* x_61; lean_object* x_62; lean_object* x_63; 
+x_61 = lean_ctor_get(x_50, 0);
+x_62 = lean_ctor_get(x_50, 1);
+lean_inc(x_62);
+lean_inc(x_61);
+lean_dec(x_50);
+x_63 = lean_alloc_ctor(1, 2, 0);
+lean_ctor_set(x_63, 0, x_61);
+lean_ctor_set(x_63, 1, x_62);
+return x_63;
+}
+}
+}
+else
+{
+uint8_t x_64; 
+lean_dec(x_8);
+lean_dec(x_7);
+lean_dec(x_6);
+lean_dec(x_5);
+lean_dec(x_1);
+x_64 = !lean_is_exclusive(x_45);
+if (x_64 == 0)
+{
+return x_45;
+}
+else
+{
+lean_object* x_65; lean_object* x_66; lean_object* x_67; 
+x_65 = lean_ctor_get(x_45, 0);
+x_66 = lean_ctor_get(x_45, 1);
+lean_inc(x_66);
+lean_inc(x_65);
+lean_dec(x_45);
+x_67 = lean_alloc_ctor(1, 2, 0);
+lean_ctor_set(x_67, 0, x_65);
+lean_ctor_set(x_67, 1, x_66);
+return x_67;
+}
+}
+}
+}
+}
+LEAN_EXPORT lean_object* l___private_Lean_Meta_Tactic_Simp_SimpTheorems_0__Lean_Meta_preprocess_go___lambda__6(uint8_t x_1, lean_object* x_2, lean_object* x_3, lean_object* x_4, lean_object* x_5, lean_object* x_6, lean_object* x_7, lean_object* x_8, lean_object* x_9, lean_object* x_10) {
 _start:
 {
 if (x_1 == 0)
@@ -6165,7 +6813,7 @@ return x_63;
 }
 }
 }
-LEAN_EXPORT lean_object* l___private_Lean_Meta_Tactic_Simp_SimpTheorems_0__Lean_Meta_preprocess_go___lambda__5(uint8_t x_1, lean_object* x_2, lean_object* x_3, lean_object* x_4, lean_object* x_5, lean_object* x_6, lean_object* x_7, lean_object* x_8, lean_object* x_9, lean_object* x_10, lean_object* x_11) {
+LEAN_EXPORT lean_object* l___private_Lean_Meta_Tactic_Simp_SimpTheorems_0__Lean_Meta_preprocess_go___lambda__7(uint8_t x_1, lean_object* x_2, lean_object* x_3, lean_object* x_4, lean_object* x_5, lean_object* x_6, lean_object* x_7, lean_object* x_8, lean_object* x_9, lean_object* x_10, lean_object* x_11) {
 _start:
 {
 if (x_1 == 0)
@@ -6300,7 +6948,7 @@ return x_38;
 }
 }
 }
-LEAN_EXPORT lean_object* l___private_Lean_Meta_Tactic_Simp_SimpTheorems_0__Lean_Meta_preprocess_go___lambda__6(lean_object* x_1, uint8_t x_2, uint8_t x_3, lean_object* x_4, lean_object* x_5, lean_object* x_6, lean_object* x_7, lean_object* x_8, lean_object* x_9, lean_object* x_10) {
+LEAN_EXPORT lean_object* l___private_Lean_Meta_Tactic_Simp_SimpTheorems_0__Lean_Meta_preprocess_go___lambda__8(lean_object* x_1, uint8_t x_2, uint8_t x_3, lean_object* x_4, lean_object* x_5, lean_object* x_6, lean_object* x_7, lean_object* x_8, lean_object* x_9, lean_object* x_10) {
 _start:
 {
 lean_object* x_11; lean_object* x_12; 
@@ -6662,7 +7310,7 @@ if (x_1 == 0)
 {
 lean_object* x_61; lean_object* x_62; 
 x_61 = lean_box(0);
-x_62 = l___private_Lean_Meta_Tactic_Simp_SimpTheorems_0__Lean_Meta_preprocess_go___lambda__2(x_60, x_3, x_61, x_5, x_6, x_7, x_8, x_12);
+x_62 = l___private_Lean_Meta_Tactic_Simp_SimpTheorems_0__Lean_Meta_preprocess_go___lambda__3(x_60, x_3, x_14, x_61, x_5, x_6, x_7, x_8, x_12);
 return x_62;
 }
 else
@@ -6709,7 +7357,7 @@ if (x_1 == 0)
 {
 lean_object* x_72; lean_object* x_73; 
 x_72 = lean_box(0);
-x_73 = l___private_Lean_Meta_Tactic_Simp_SimpTheorems_0__Lean_Meta_preprocess_go___lambda__3(x_70, x_71, x_3, x_72, x_5, x_6, x_7, x_8, x_12);
+x_73 = l___private_Lean_Meta_Tactic_Simp_SimpTheorems_0__Lean_Meta_preprocess_go___lambda__5(x_70, x_71, x_3, x_72, x_5, x_6, x_7, x_8, x_12);
 return x_73;
 }
 else
@@ -6757,7 +7405,7 @@ if (x_2 == 0)
 {
 lean_object* x_83; lean_object* x_84; 
 x_83 = lean_box(0);
-x_84 = l___private_Lean_Meta_Tactic_Simp_SimpTheorems_0__Lean_Meta_preprocess_go___lambda__4(x_1, x_81, x_82, x_3, x_83, x_5, x_6, x_7, x_8, x_12);
+x_84 = l___private_Lean_Meta_Tactic_Simp_SimpTheorems_0__Lean_Meta_preprocess_go___lambda__6(x_1, x_81, x_82, x_3, x_83, x_5, x_6, x_7, x_8, x_12);
 return x_84;
 }
 else
@@ -6778,7 +7426,7 @@ lean_inc(x_86);
 x_87 = lean_ctor_get(x_85, 1);
 lean_inc(x_87);
 lean_dec(x_85);
-x_88 = l___private_Lean_Meta_Tactic_Simp_SimpTheorems_0__Lean_Meta_preprocess_go___lambda__4(x_1, x_81, x_82, x_3, x_86, x_5, x_6, x_7, x_8, x_87);
+x_88 = l___private_Lean_Meta_Tactic_Simp_SimpTheorems_0__Lean_Meta_preprocess_go___lambda__6(x_1, x_81, x_82, x_3, x_86, x_5, x_6, x_7, x_8, x_87);
 lean_dec(x_86);
 return x_88;
 }
@@ -6825,7 +7473,7 @@ if (x_2 == 0)
 {
 lean_object* x_96; lean_object* x_97; 
 x_96 = lean_box(0);
-x_97 = l___private_Lean_Meta_Tactic_Simp_SimpTheorems_0__Lean_Meta_preprocess_go___lambda__5(x_1, x_3, x_11, x_95, x_94, x_96, x_5, x_6, x_7, x_8, x_12);
+x_97 = l___private_Lean_Meta_Tactic_Simp_SimpTheorems_0__Lean_Meta_preprocess_go___lambda__7(x_1, x_3, x_11, x_95, x_94, x_96, x_5, x_6, x_7, x_8, x_12);
 return x_97;
 }
 else
@@ -6846,7 +7494,7 @@ lean_inc(x_99);
 x_100 = lean_ctor_get(x_98, 1);
 lean_inc(x_100);
 lean_dec(x_98);
-x_101 = l___private_Lean_Meta_Tactic_Simp_SimpTheorems_0__Lean_Meta_preprocess_go___lambda__5(x_1, x_3, x_11, x_95, x_94, x_99, x_5, x_6, x_7, x_8, x_100);
+x_101 = l___private_Lean_Meta_Tactic_Simp_SimpTheorems_0__Lean_Meta_preprocess_go___lambda__7(x_1, x_3, x_11, x_95, x_94, x_99, x_5, x_6, x_7, x_8, x_100);
 lean_dec(x_99);
 return x_101;
 }
@@ -6888,7 +7536,7 @@ else
 lean_object* x_106; lean_object* x_107; lean_object* x_108; lean_object* x_109; 
 x_106 = lean_box(x_1);
 x_107 = lean_box(x_2);
-x_108 = lean_alloc_closure((void*)(l___private_Lean_Meta_Tactic_Simp_SimpTheorems_0__Lean_Meta_preprocess_go___lambda__6___boxed), 10, 3);
+x_108 = lean_alloc_closure((void*)(l___private_Lean_Meta_Tactic_Simp_SimpTheorems_0__Lean_Meta_preprocess_go___lambda__8___boxed), 10, 3);
 lean_closure_set(x_108, 0, x_3);
 lean_closure_set(x_108, 1, x_106);
 lean_closure_set(x_108, 2, x_107);
@@ -6954,38 +7602,38 @@ lean_dec(x_3);
 return x_9;
 }
 }
-LEAN_EXPORT lean_object* l___private_Lean_Meta_Tactic_Simp_SimpTheorems_0__Lean_Meta_preprocess_go___lambda__3___boxed(lean_object* x_1, lean_object* x_2, lean_object* x_3, lean_object* x_4, lean_object* x_5, lean_object* x_6, lean_object* x_7, lean_object* x_8, lean_object* x_9) {
+LEAN_EXPORT lean_object* l___private_Lean_Meta_Tactic_Simp_SimpTheorems_0__Lean_Meta_preprocess_go___lambda__4___boxed(lean_object* x_1, lean_object* x_2, lean_object* x_3, lean_object* x_4, lean_object* x_5, lean_object* x_6, lean_object* x_7, lean_object* x_8, lean_object* x_9) {
 _start:
 {
 lean_object* x_10; 
-x_10 = l___private_Lean_Meta_Tactic_Simp_SimpTheorems_0__Lean_Meta_preprocess_go___lambda__3(x_1, x_2, x_3, x_4, x_5, x_6, x_7, x_8, x_9);
+x_10 = l___private_Lean_Meta_Tactic_Simp_SimpTheorems_0__Lean_Meta_preprocess_go___lambda__4(x_1, x_2, x_3, x_4, x_5, x_6, x_7, x_8, x_9);
 lean_dec(x_4);
 return x_10;
 }
 }
-LEAN_EXPORT lean_object* l___private_Lean_Meta_Tactic_Simp_SimpTheorems_0__Lean_Meta_preprocess_go___lambda__4___boxed(lean_object* x_1, lean_object* x_2, lean_object* x_3, lean_object* x_4, lean_object* x_5, lean_object* x_6, lean_object* x_7, lean_object* x_8, lean_object* x_9, lean_object* x_10) {
+LEAN_EXPORT lean_object* l___private_Lean_Meta_Tactic_Simp_SimpTheorems_0__Lean_Meta_preprocess_go___lambda__6___boxed(lean_object* x_1, lean_object* x_2, lean_object* x_3, lean_object* x_4, lean_object* x_5, lean_object* x_6, lean_object* x_7, lean_object* x_8, lean_object* x_9, lean_object* x_10) {
 _start:
 {
 uint8_t x_11; lean_object* x_12; 
 x_11 = lean_unbox(x_1);
 lean_dec(x_1);
-x_12 = l___private_Lean_Meta_Tactic_Simp_SimpTheorems_0__Lean_Meta_preprocess_go___lambda__4(x_11, x_2, x_3, x_4, x_5, x_6, x_7, x_8, x_9, x_10);
+x_12 = l___private_Lean_Meta_Tactic_Simp_SimpTheorems_0__Lean_Meta_preprocess_go___lambda__6(x_11, x_2, x_3, x_4, x_5, x_6, x_7, x_8, x_9, x_10);
 lean_dec(x_5);
 return x_12;
 }
 }
-LEAN_EXPORT lean_object* l___private_Lean_Meta_Tactic_Simp_SimpTheorems_0__Lean_Meta_preprocess_go___lambda__5___boxed(lean_object* x_1, lean_object* x_2, lean_object* x_3, lean_object* x_4, lean_object* x_5, lean_object* x_6, lean_object* x_7, lean_object* x_8, lean_object* x_9, lean_object* x_10, lean_object* x_11) {
+LEAN_EXPORT lean_object* l___private_Lean_Meta_Tactic_Simp_SimpTheorems_0__Lean_Meta_preprocess_go___lambda__7___boxed(lean_object* x_1, lean_object* x_2, lean_object* x_3, lean_object* x_4, lean_object* x_5, lean_object* x_6, lean_object* x_7, lean_object* x_8, lean_object* x_9, lean_object* x_10, lean_object* x_11) {
 _start:
 {
 uint8_t x_12; lean_object* x_13; 
 x_12 = lean_unbox(x_1);
 lean_dec(x_1);
-x_13 = l___private_Lean_Meta_Tactic_Simp_SimpTheorems_0__Lean_Meta_preprocess_go___lambda__5(x_12, x_2, x_3, x_4, x_5, x_6, x_7, x_8, x_9, x_10, x_11);
+x_13 = l___private_Lean_Meta_Tactic_Simp_SimpTheorems_0__Lean_Meta_preprocess_go___lambda__7(x_12, x_2, x_3, x_4, x_5, x_6, x_7, x_8, x_9, x_10, x_11);
 lean_dec(x_6);
 return x_13;
 }
 }
-LEAN_EXPORT lean_object* l___private_Lean_Meta_Tactic_Simp_SimpTheorems_0__Lean_Meta_preprocess_go___lambda__6___boxed(lean_object* x_1, lean_object* x_2, lean_object* x_3, lean_object* x_4, lean_object* x_5, lean_object* x_6, lean_object* x_7, lean_object* x_8, lean_object* x_9, lean_object* x_10) {
+LEAN_EXPORT lean_object* l___private_Lean_Meta_Tactic_Simp_SimpTheorems_0__Lean_Meta_preprocess_go___lambda__8___boxed(lean_object* x_1, lean_object* x_2, lean_object* x_3, lean_object* x_4, lean_object* x_5, lean_object* x_6, lean_object* x_7, lean_object* x_8, lean_object* x_9, lean_object* x_10) {
 _start:
 {
 uint8_t x_11; uint8_t x_12; lean_object* x_13; 
@@ -6993,7 +7641,7 @@ x_11 = lean_unbox(x_2);
 lean_dec(x_2);
 x_12 = lean_unbox(x_3);
 lean_dec(x_3);
-x_13 = l___private_Lean_Meta_Tactic_Simp_SimpTheorems_0__Lean_Meta_preprocess_go___lambda__6(x_1, x_11, x_12, x_4, x_5, x_6, x_7, x_8, x_9, x_10);
+x_13 = l___private_Lean_Meta_Tactic_Simp_SimpTheorems_0__Lean_Meta_preprocess_go___lambda__8(x_1, x_11, x_12, x_4, x_5, x_6, x_7, x_8, x_9, x_10);
 return x_13;
 }
 }
@@ -8301,15 +8949,6 @@ return x_38;
 }
 }
 }
-static lean_object* _init_l___private_Lean_Meta_Tactic_Simp_SimpTheorems_0__Lean_Meta_mkSimpTheoremsFromConst___closed__1() {
-_start:
-{
-lean_object* x_1; lean_object* x_2; 
-x_1 = lean_unsigned_to_nat(1u);
-x_2 = lean_mk_empty_array_with_capacity(x_1);
-return x_2;
-}
-}
 LEAN_EXPORT lean_object* l___private_Lean_Meta_Tactic_Simp_SimpTheorems_0__Lean_Meta_mkSimpTheoremsFromConst(lean_object* x_1, uint8_t x_2, uint8_t x_3, lean_object* x_4, lean_object* x_5, lean_object* x_6, lean_object* x_7, lean_object* x_8, lean_object* x_9) {
 _start:
 {
@@ -8409,7 +9048,7 @@ if (x_55 == 0)
 {
 lean_object* x_56; lean_object* x_57; lean_object* x_58; 
 x_56 = lean_ctor_get(x_54, 0);
-x_57 = l___private_Lean_Meta_Tactic_Simp_SimpTheorems_0__Lean_Meta_mkSimpTheoremsFromConst___closed__1;
+x_57 = l___private_Lean_Meta_Tactic_Simp_SimpTheorems_0__Lean_Meta_preprocess_go___lambda__3___closed__9;
 x_58 = lean_array_push(x_57, x_56);
 lean_ctor_set(x_54, 0, x_58);
 return x_54;
@@ -8422,7 +9061,7 @@ x_60 = lean_ctor_get(x_54, 1);
 lean_inc(x_60);
 lean_inc(x_59);
 lean_dec(x_54);
-x_61 = l___private_Lean_Meta_Tactic_Simp_SimpTheorems_0__Lean_Meta_mkSimpTheoremsFromConst___closed__1;
+x_61 = l___private_Lean_Meta_Tactic_Simp_SimpTheorems_0__Lean_Meta_preprocess_go___lambda__3___closed__9;
 x_62 = lean_array_push(x_61, x_59);
 x_63 = lean_alloc_ctor(0, 2, 0);
 lean_ctor_set(x_63, 0, x_62);
@@ -8771,7 +9410,7 @@ if (lean_is_exclusive(x_130)) {
  lean_dec_ref(x_130);
  x_133 = lean_box(0);
 }
-x_134 = l___private_Lean_Meta_Tactic_Simp_SimpTheorems_0__Lean_Meta_mkSimpTheoremsFromConst___closed__1;
+x_134 = l___private_Lean_Meta_Tactic_Simp_SimpTheorems_0__Lean_Meta_preprocess_go___lambda__3___closed__9;
 x_135 = lean_array_push(x_134, x_131);
 if (lean_is_scalar(x_133)) {
  x_136 = lean_alloc_ctor(0, 2, 0);
@@ -9166,7 +9805,7 @@ if (lean_is_exclusive(x_211)) {
  lean_dec_ref(x_211);
  x_214 = lean_box(0);
 }
-x_215 = l___private_Lean_Meta_Tactic_Simp_SimpTheorems_0__Lean_Meta_mkSimpTheoremsFromConst___closed__1;
+x_215 = l___private_Lean_Meta_Tactic_Simp_SimpTheorems_0__Lean_Meta_preprocess_go___lambda__3___closed__9;
 x_216 = lean_array_push(x_215, x_212);
 if (lean_is_scalar(x_214)) {
  x_217 = lean_alloc_ctor(0, 2, 0);
@@ -11357,7 +11996,7 @@ return x_20;
 }
 }
 }
-static lean_object* _init_l_Lean_Meta_initFn____x40_Lean_Meta_Tactic_Simp_SimpTheorems___hyg_3740____closed__1() {
+static lean_object* _init_l_Lean_Meta_initFn____x40_Lean_Meta_Tactic_Simp_SimpTheorems___hyg_4092____closed__1() {
 _start:
 {
 lean_object* x_1; 
@@ -11365,17 +12004,17 @@ x_1 = lean_mk_string("simp");
 return x_1;
 }
 }
-static lean_object* _init_l_Lean_Meta_initFn____x40_Lean_Meta_Tactic_Simp_SimpTheorems___hyg_3740____closed__2() {
+static lean_object* _init_l_Lean_Meta_initFn____x40_Lean_Meta_Tactic_Simp_SimpTheorems___hyg_4092____closed__2() {
 _start:
 {
 lean_object* x_1; lean_object* x_2; lean_object* x_3; 
 x_1 = lean_box(0);
-x_2 = l_Lean_Meta_initFn____x40_Lean_Meta_Tactic_Simp_SimpTheorems___hyg_3740____closed__1;
+x_2 = l_Lean_Meta_initFn____x40_Lean_Meta_Tactic_Simp_SimpTheorems___hyg_4092____closed__1;
 x_3 = lean_name_mk_string(x_1, x_2);
 return x_3;
 }
 }
-static lean_object* _init_l_Lean_Meta_initFn____x40_Lean_Meta_Tactic_Simp_SimpTheorems___hyg_3740____closed__3() {
+static lean_object* _init_l_Lean_Meta_initFn____x40_Lean_Meta_Tactic_Simp_SimpTheorems___hyg_4092____closed__3() {
 _start:
 {
 lean_object* x_1; 
@@ -11383,17 +12022,17 @@ x_1 = lean_mk_string("Ext");
 return x_1;
 }
 }
-static lean_object* _init_l_Lean_Meta_initFn____x40_Lean_Meta_Tactic_Simp_SimpTheorems___hyg_3740____closed__4() {
+static lean_object* _init_l_Lean_Meta_initFn____x40_Lean_Meta_Tactic_Simp_SimpTheorems___hyg_4092____closed__4() {
 _start:
 {
 lean_object* x_1; lean_object* x_2; lean_object* x_3; 
-x_1 = l_Lean_Meta_initFn____x40_Lean_Meta_Tactic_Simp_SimpTheorems___hyg_3740____closed__2;
-x_2 = l_Lean_Meta_initFn____x40_Lean_Meta_Tactic_Simp_SimpTheorems___hyg_3740____closed__3;
+x_1 = l_Lean_Meta_initFn____x40_Lean_Meta_Tactic_Simp_SimpTheorems___hyg_4092____closed__2;
+x_2 = l_Lean_Meta_initFn____x40_Lean_Meta_Tactic_Simp_SimpTheorems___hyg_4092____closed__3;
 x_3 = lean_name_append_after(x_1, x_2);
 return x_3;
 }
 }
-static lean_object* _init_l_Lean_Meta_initFn____x40_Lean_Meta_Tactic_Simp_SimpTheorems___hyg_3740____closed__5() {
+static lean_object* _init_l_Lean_Meta_initFn____x40_Lean_Meta_Tactic_Simp_SimpTheorems___hyg_4092____closed__5() {
 _start:
 {
 lean_object* x_1; 
@@ -11401,13 +12040,13 @@ x_1 = lean_mk_string("simplification theorem");
 return x_1;
 }
 }
-LEAN_EXPORT lean_object* l_Lean_Meta_initFn____x40_Lean_Meta_Tactic_Simp_SimpTheorems___hyg_3740_(lean_object* x_1) {
+LEAN_EXPORT lean_object* l_Lean_Meta_initFn____x40_Lean_Meta_Tactic_Simp_SimpTheorems___hyg_4092_(lean_object* x_1) {
 _start:
 {
 lean_object* x_2; lean_object* x_3; lean_object* x_4; lean_object* x_5; 
-x_2 = l_Lean_Meta_initFn____x40_Lean_Meta_Tactic_Simp_SimpTheorems___hyg_3740____closed__2;
-x_3 = l_Lean_Meta_initFn____x40_Lean_Meta_Tactic_Simp_SimpTheorems___hyg_3740____closed__5;
-x_4 = l_Lean_Meta_initFn____x40_Lean_Meta_Tactic_Simp_SimpTheorems___hyg_3740____closed__4;
+x_2 = l_Lean_Meta_initFn____x40_Lean_Meta_Tactic_Simp_SimpTheorems___hyg_4092____closed__2;
+x_3 = l_Lean_Meta_initFn____x40_Lean_Meta_Tactic_Simp_SimpTheorems___hyg_4092____closed__5;
+x_4 = l_Lean_Meta_initFn____x40_Lean_Meta_Tactic_Simp_SimpTheorems___hyg_4092____closed__4;
 x_5 = l_Lean_Meta_registerSimpAttr(x_2, x_3, x_4, x_1);
 return x_5;
 }
@@ -13601,6 +14240,32 @@ l___private_Lean_Meta_Tactic_Simp_SimpTheorems_0__Lean_Meta_preprocess_go___lamb
 lean_mark_persistent(l___private_Lean_Meta_Tactic_Simp_SimpTheorems_0__Lean_Meta_preprocess_go___lambda__2___closed__2);
 l___private_Lean_Meta_Tactic_Simp_SimpTheorems_0__Lean_Meta_preprocess_go___lambda__2___closed__3 = _init_l___private_Lean_Meta_Tactic_Simp_SimpTheorems_0__Lean_Meta_preprocess_go___lambda__2___closed__3();
 lean_mark_persistent(l___private_Lean_Meta_Tactic_Simp_SimpTheorems_0__Lean_Meta_preprocess_go___lambda__2___closed__3);
+l___private_Lean_Meta_Tactic_Simp_SimpTheorems_0__Lean_Meta_preprocess_go___lambda__3___closed__1 = _init_l___private_Lean_Meta_Tactic_Simp_SimpTheorems_0__Lean_Meta_preprocess_go___lambda__3___closed__1();
+lean_mark_persistent(l___private_Lean_Meta_Tactic_Simp_SimpTheorems_0__Lean_Meta_preprocess_go___lambda__3___closed__1);
+l___private_Lean_Meta_Tactic_Simp_SimpTheorems_0__Lean_Meta_preprocess_go___lambda__3___closed__2 = _init_l___private_Lean_Meta_Tactic_Simp_SimpTheorems_0__Lean_Meta_preprocess_go___lambda__3___closed__2();
+lean_mark_persistent(l___private_Lean_Meta_Tactic_Simp_SimpTheorems_0__Lean_Meta_preprocess_go___lambda__3___closed__2);
+l___private_Lean_Meta_Tactic_Simp_SimpTheorems_0__Lean_Meta_preprocess_go___lambda__3___closed__3 = _init_l___private_Lean_Meta_Tactic_Simp_SimpTheorems_0__Lean_Meta_preprocess_go___lambda__3___closed__3();
+lean_mark_persistent(l___private_Lean_Meta_Tactic_Simp_SimpTheorems_0__Lean_Meta_preprocess_go___lambda__3___closed__3);
+l___private_Lean_Meta_Tactic_Simp_SimpTheorems_0__Lean_Meta_preprocess_go___lambda__3___closed__4 = _init_l___private_Lean_Meta_Tactic_Simp_SimpTheorems_0__Lean_Meta_preprocess_go___lambda__3___closed__4();
+lean_mark_persistent(l___private_Lean_Meta_Tactic_Simp_SimpTheorems_0__Lean_Meta_preprocess_go___lambda__3___closed__4);
+l___private_Lean_Meta_Tactic_Simp_SimpTheorems_0__Lean_Meta_preprocess_go___lambda__3___closed__5 = _init_l___private_Lean_Meta_Tactic_Simp_SimpTheorems_0__Lean_Meta_preprocess_go___lambda__3___closed__5();
+lean_mark_persistent(l___private_Lean_Meta_Tactic_Simp_SimpTheorems_0__Lean_Meta_preprocess_go___lambda__3___closed__5);
+l___private_Lean_Meta_Tactic_Simp_SimpTheorems_0__Lean_Meta_preprocess_go___lambda__3___closed__6 = _init_l___private_Lean_Meta_Tactic_Simp_SimpTheorems_0__Lean_Meta_preprocess_go___lambda__3___closed__6();
+lean_mark_persistent(l___private_Lean_Meta_Tactic_Simp_SimpTheorems_0__Lean_Meta_preprocess_go___lambda__3___closed__6);
+l___private_Lean_Meta_Tactic_Simp_SimpTheorems_0__Lean_Meta_preprocess_go___lambda__3___closed__7 = _init_l___private_Lean_Meta_Tactic_Simp_SimpTheorems_0__Lean_Meta_preprocess_go___lambda__3___closed__7();
+lean_mark_persistent(l___private_Lean_Meta_Tactic_Simp_SimpTheorems_0__Lean_Meta_preprocess_go___lambda__3___closed__7);
+l___private_Lean_Meta_Tactic_Simp_SimpTheorems_0__Lean_Meta_preprocess_go___lambda__3___closed__8 = _init_l___private_Lean_Meta_Tactic_Simp_SimpTheorems_0__Lean_Meta_preprocess_go___lambda__3___closed__8();
+lean_mark_persistent(l___private_Lean_Meta_Tactic_Simp_SimpTheorems_0__Lean_Meta_preprocess_go___lambda__3___closed__8);
+l___private_Lean_Meta_Tactic_Simp_SimpTheorems_0__Lean_Meta_preprocess_go___lambda__3___closed__9 = _init_l___private_Lean_Meta_Tactic_Simp_SimpTheorems_0__Lean_Meta_preprocess_go___lambda__3___closed__9();
+lean_mark_persistent(l___private_Lean_Meta_Tactic_Simp_SimpTheorems_0__Lean_Meta_preprocess_go___lambda__3___closed__9);
+l___private_Lean_Meta_Tactic_Simp_SimpTheorems_0__Lean_Meta_preprocess_go___lambda__3___closed__10 = _init_l___private_Lean_Meta_Tactic_Simp_SimpTheorems_0__Lean_Meta_preprocess_go___lambda__3___closed__10();
+lean_mark_persistent(l___private_Lean_Meta_Tactic_Simp_SimpTheorems_0__Lean_Meta_preprocess_go___lambda__3___closed__10);
+l___private_Lean_Meta_Tactic_Simp_SimpTheorems_0__Lean_Meta_preprocess_go___lambda__3___closed__11 = _init_l___private_Lean_Meta_Tactic_Simp_SimpTheorems_0__Lean_Meta_preprocess_go___lambda__3___closed__11();
+lean_mark_persistent(l___private_Lean_Meta_Tactic_Simp_SimpTheorems_0__Lean_Meta_preprocess_go___lambda__3___closed__11);
+l___private_Lean_Meta_Tactic_Simp_SimpTheorems_0__Lean_Meta_preprocess_go___lambda__3___closed__12 = _init_l___private_Lean_Meta_Tactic_Simp_SimpTheorems_0__Lean_Meta_preprocess_go___lambda__3___closed__12();
+lean_mark_persistent(l___private_Lean_Meta_Tactic_Simp_SimpTheorems_0__Lean_Meta_preprocess_go___lambda__3___closed__12);
+l___private_Lean_Meta_Tactic_Simp_SimpTheorems_0__Lean_Meta_preprocess_go___lambda__3___closed__13 = _init_l___private_Lean_Meta_Tactic_Simp_SimpTheorems_0__Lean_Meta_preprocess_go___lambda__3___closed__13();
+lean_mark_persistent(l___private_Lean_Meta_Tactic_Simp_SimpTheorems_0__Lean_Meta_preprocess_go___lambda__3___closed__13);
 l___private_Lean_Meta_Tactic_Simp_SimpTheorems_0__Lean_Meta_preprocess_go___closed__1 = _init_l___private_Lean_Meta_Tactic_Simp_SimpTheorems_0__Lean_Meta_preprocess_go___closed__1();
 lean_mark_persistent(l___private_Lean_Meta_Tactic_Simp_SimpTheorems_0__Lean_Meta_preprocess_go___closed__1);
 l___private_Lean_Meta_Tactic_Simp_SimpTheorems_0__Lean_Meta_preprocess_go___closed__2 = _init_l___private_Lean_Meta_Tactic_Simp_SimpTheorems_0__Lean_Meta_preprocess_go___closed__2();
@@ -13633,8 +14298,6 @@ l___private_Lean_Meta_Tactic_Simp_SimpTheorems_0__Lean_Meta_mkSimpTheoremCore___
 lean_mark_persistent(l___private_Lean_Meta_Tactic_Simp_SimpTheorems_0__Lean_Meta_mkSimpTheoremCore___lambda__2___closed__1);
 l___private_Lean_Meta_Tactic_Simp_SimpTheorems_0__Lean_Meta_mkSimpTheoremCore___lambda__2___closed__2 = _init_l___private_Lean_Meta_Tactic_Simp_SimpTheorems_0__Lean_Meta_mkSimpTheoremCore___lambda__2___closed__2();
 lean_mark_persistent(l___private_Lean_Meta_Tactic_Simp_SimpTheorems_0__Lean_Meta_mkSimpTheoremCore___lambda__2___closed__2);
-l___private_Lean_Meta_Tactic_Simp_SimpTheorems_0__Lean_Meta_mkSimpTheoremsFromConst___closed__1 = _init_l___private_Lean_Meta_Tactic_Simp_SimpTheorems_0__Lean_Meta_mkSimpTheoremsFromConst___closed__1();
-lean_mark_persistent(l___private_Lean_Meta_Tactic_Simp_SimpTheorems_0__Lean_Meta_mkSimpTheoremsFromConst___closed__1);
 l_Lean_Meta_instInhabitedSimpEntry___closed__1 = _init_l_Lean_Meta_instInhabitedSimpEntry___closed__1();
 lean_mark_persistent(l_Lean_Meta_instInhabitedSimpEntry___closed__1);
 l_Lean_Meta_instInhabitedSimpEntry = _init_l_Lean_Meta_instInhabitedSimpEntry();
@@ -13701,17 +14364,17 @@ l_Lean_Meta_mkSimpExt___closed__2 = _init_l_Lean_Meta_mkSimpExt___closed__2();
 lean_mark_persistent(l_Lean_Meta_mkSimpExt___closed__2);
 l_Lean_Meta_mkSimpExt___closed__3 = _init_l_Lean_Meta_mkSimpExt___closed__3();
 lean_mark_persistent(l_Lean_Meta_mkSimpExt___closed__3);
-l_Lean_Meta_initFn____x40_Lean_Meta_Tactic_Simp_SimpTheorems___hyg_3740____closed__1 = _init_l_Lean_Meta_initFn____x40_Lean_Meta_Tactic_Simp_SimpTheorems___hyg_3740____closed__1();
-lean_mark_persistent(l_Lean_Meta_initFn____x40_Lean_Meta_Tactic_Simp_SimpTheorems___hyg_3740____closed__1);
-l_Lean_Meta_initFn____x40_Lean_Meta_Tactic_Simp_SimpTheorems___hyg_3740____closed__2 = _init_l_Lean_Meta_initFn____x40_Lean_Meta_Tactic_Simp_SimpTheorems___hyg_3740____closed__2();
-lean_mark_persistent(l_Lean_Meta_initFn____x40_Lean_Meta_Tactic_Simp_SimpTheorems___hyg_3740____closed__2);
-l_Lean_Meta_initFn____x40_Lean_Meta_Tactic_Simp_SimpTheorems___hyg_3740____closed__3 = _init_l_Lean_Meta_initFn____x40_Lean_Meta_Tactic_Simp_SimpTheorems___hyg_3740____closed__3();
-lean_mark_persistent(l_Lean_Meta_initFn____x40_Lean_Meta_Tactic_Simp_SimpTheorems___hyg_3740____closed__3);
-l_Lean_Meta_initFn____x40_Lean_Meta_Tactic_Simp_SimpTheorems___hyg_3740____closed__4 = _init_l_Lean_Meta_initFn____x40_Lean_Meta_Tactic_Simp_SimpTheorems___hyg_3740____closed__4();
-lean_mark_persistent(l_Lean_Meta_initFn____x40_Lean_Meta_Tactic_Simp_SimpTheorems___hyg_3740____closed__4);
-l_Lean_Meta_initFn____x40_Lean_Meta_Tactic_Simp_SimpTheorems___hyg_3740____closed__5 = _init_l_Lean_Meta_initFn____x40_Lean_Meta_Tactic_Simp_SimpTheorems___hyg_3740____closed__5();
-lean_mark_persistent(l_Lean_Meta_initFn____x40_Lean_Meta_Tactic_Simp_SimpTheorems___hyg_3740____closed__5);
-if (builtin) {res = l_Lean_Meta_initFn____x40_Lean_Meta_Tactic_Simp_SimpTheorems___hyg_3740_(lean_io_mk_world());
+l_Lean_Meta_initFn____x40_Lean_Meta_Tactic_Simp_SimpTheorems___hyg_4092____closed__1 = _init_l_Lean_Meta_initFn____x40_Lean_Meta_Tactic_Simp_SimpTheorems___hyg_4092____closed__1();
+lean_mark_persistent(l_Lean_Meta_initFn____x40_Lean_Meta_Tactic_Simp_SimpTheorems___hyg_4092____closed__1);
+l_Lean_Meta_initFn____x40_Lean_Meta_Tactic_Simp_SimpTheorems___hyg_4092____closed__2 = _init_l_Lean_Meta_initFn____x40_Lean_Meta_Tactic_Simp_SimpTheorems___hyg_4092____closed__2();
+lean_mark_persistent(l_Lean_Meta_initFn____x40_Lean_Meta_Tactic_Simp_SimpTheorems___hyg_4092____closed__2);
+l_Lean_Meta_initFn____x40_Lean_Meta_Tactic_Simp_SimpTheorems___hyg_4092____closed__3 = _init_l_Lean_Meta_initFn____x40_Lean_Meta_Tactic_Simp_SimpTheorems___hyg_4092____closed__3();
+lean_mark_persistent(l_Lean_Meta_initFn____x40_Lean_Meta_Tactic_Simp_SimpTheorems___hyg_4092____closed__3);
+l_Lean_Meta_initFn____x40_Lean_Meta_Tactic_Simp_SimpTheorems___hyg_4092____closed__4 = _init_l_Lean_Meta_initFn____x40_Lean_Meta_Tactic_Simp_SimpTheorems___hyg_4092____closed__4();
+lean_mark_persistent(l_Lean_Meta_initFn____x40_Lean_Meta_Tactic_Simp_SimpTheorems___hyg_4092____closed__4);
+l_Lean_Meta_initFn____x40_Lean_Meta_Tactic_Simp_SimpTheorems___hyg_4092____closed__5 = _init_l_Lean_Meta_initFn____x40_Lean_Meta_Tactic_Simp_SimpTheorems___hyg_4092____closed__5();
+lean_mark_persistent(l_Lean_Meta_initFn____x40_Lean_Meta_Tactic_Simp_SimpTheorems___hyg_4092____closed__5);
+if (builtin) {res = l_Lean_Meta_initFn____x40_Lean_Meta_Tactic_Simp_SimpTheorems___hyg_4092_(lean_io_mk_world());
 if (lean_io_result_is_error(res)) return res;
 l_Lean_Meta_simpExtension = lean_io_result_get_value(res);
 lean_mark_persistent(l_Lean_Meta_simpExtension);
