stage0/src/Init/SimpLemmas.lean
@@ -139,6 +139,10 @@ theorem dite_congr {s : Decidable b} [Decidable c]
 
 @[simp] theorem Bool.beq_to_eq (a b : Bool) : ((a == b) = true) = (a = b) := by cases a <;> cases b <;> decide
 @[simp] theorem Bool.not_beq_to_not_eq (a b : Bool) : ((!(a == b)) = true) = ¬(a = b) := by cases a <;> cases b <;> decide
+
+theorem Bool.of_not_eq_true {b : Bool} : ¬ (b = true) → b = false := by cases b <;> decide
+theorem Bool.of_not_eq_false {b : Bool} : ¬ (b = false) → b = true := by cases b <;> decide
+
 @[simp] theorem Bool.not_eq_true (b : Bool) : (¬ (b = true)) = (b = false) := by cases b <;> decide
 @[simp] theorem Bool.not_eq_false (b : Bool) : (¬ (b = false)) = (b = true) := by cases b <;> decide
 
@@ -150,3 +154,6 @@ theorem dite_congr {s : Decidable b} [Decidable c]
 @[simp] theorem Nat.not_beq_to_not_eq (a b : Nat) : ((!(a == b)) = true) = ¬(a = b) := by simp [BEq.beq]
 
 @[simp] theorem heq_eq_eq {α : Sort u} (a b : α) : HEq a b = (a = b) := propext <| Iff.intro eq_of_heq heq_of_eq
+
+@[simp] theorem cond_true (a b : α) : cond true a b = a := rfl
+@[simp] theorem cond_false (a b : α) : cond false a b = b := rfl
